Rename constructors in ILC

thys/Infinitary_Lambda_Calculus/ILC.thy
@@ -45,10 +45,10 @@ declare [[inductive_internals]]
 declare [[mrbnf_internals]]
 
 (*infinitary untyped lambda calculus*)
-binder_datatype 'a iterm
-  = iVar 'a
-  | iApp "'a iterm" "'a iterm stream"
-  | iLam "(xs::'a) dstream" t::"'a iterm" binds xs in t
+binder_datatype (iFV: 'var) iterm
+  = iVr 'var
+  | iAp "'var iterm" "'var iterm stream"
+  | iLm "(xs::'var) dstream" t::"'var iterm" binds xs in t
 for
   vvsubst: ivvsubst
   tvsubst: itvsubst
@@ -154,14 +154,13 @@ abbreviation "IImsupp \<equiv> IImsupp_iterm"
 lemmas IImsupp_def = IImsupp_iterm_def
 abbreviation "SSupp \<equiv> SSupp_iterm"
 lemmas SSupp_def = SSupp_iterm_def
-abbreviation "FFVars \<equiv> FVars_iterm"
 
 abbreviation "irrename \<equiv> permute_iterm"
 (* *)
 
-lemma FFVars_itvsubst[simp]:
+lemma iFV_itvsubst[simp]:
   assumes "|SSupp (\<sigma> :: ivar \<Rightarrow> itrm)| <o |UNIV :: ivar set|"
-  shows "FFVars (itvsubst \<sigma> t) = (\<Union> {FFVars (\<sigma> x) | x . x \<in> FFVars t})"
+  shows "iFV (itvsubst \<sigma> t) = (\<Union> {iFV (\<sigma> x) | x . x \<in> iFV t})"
   apply (binder_induction t avoiding: "IImsupp \<sigma>" rule: iterm.strong_induct)
   apply (rule iterm.fresh_induct[of "IImsupp \<sigma>"])
      apply (auto simp: IImsupp_def assms intro!: Un_bound UN_bound iterm.set_bd_UNIV)
@@ -193,9 +192,9 @@ lemma IImsupp_VVr_empty[simp]: "IImsupp VVr = {}"
   apply (rule refl)
   done
 
-(* VVr is here the Var constructor: *)
-lemma VVr_eq_Var[simp]: "VVr = iVar"
-  unfolding VVr_def iVar_def comp_def
+(* VVr is here the Vrconstructor: *)
+lemma VVr_eq_Var[simp]: "VVr = iVr"
+  unfolding VVr_def iVr_def comp_def
   tv\<eta>_iterm_itvsubst_def
   by (rule refl)
 
@@ -237,20 +236,20 @@ lemmas iterm.inject(3)[simp del]
 
 lemma itvsubst_cong:
 assumes f: "|SSupp f| <o |UNIV::ivar set|" and g: "|SSupp g| <o |UNIV::ivar set|"
-and eq: "(\<And>z. (z::ivar) \<in> FFVars P \<Longrightarrow> f z = g z)"
+and eq: "(\<And>z. (z::ivar) \<in> iFV P \<Longrightarrow> f z = g z)"
 shows "itvsubst f P = itvsubst g P"
 using eq proof (binder_induction P avoiding: "IImsupp f" "IImsupp g" rule: iterm.strong_induct)
-  case (iApp x1 x2)
+  case (iAp x1 x2)
   then show ?case using f g by simp (metis stream.map_cong0)
 next
-  case (iLam x1 x2)
+  case (iLm x1 x2)
   then show ?case  using f g apply simp
     by (smt (verit, ccfv_threshold) IImsupp_def SSupp_def UnCI insert_absorb insert_disjoint(2) mem_Collect_eq)
 qed (auto simp: IImsupp_def iterm.UN_bound iterm.Un_bound iterm.set_bd_UNIV f g)
 
 (* *)
 
-lemma iLam_same_inject[simp]: "iLam (xs::ivar dstream) e = iLam xs e' \<longleftrightarrow> e = e'"
+lemma iLm_same_inject[simp]: "iLm (xs::ivar dstream) e = iLm xs e' \<longleftrightarrow> e = e'"
 unfolding iterm.inject apply safe
 apply(rule iterm.permute_cong_id[symmetric])
 unfolding id_on_def by auto (metis bij_betw_def bij_imp_bij_betw dsnth_dsmap dtheN)
@@ -291,9 +290,9 @@ lemma map_term_pre_inv_simp: "bij f \<Longrightarrow> |supp (f::ivar \<Rightarro
    apply (rule refl)+
   done
 
-lemma iLam_set3: "iterm_ctor v = iLam (xs::ivar dstream) e \<Longrightarrow>
- \<exists>xs' e'. iterm_ctor v = iLam xs' e' \<and> dsset xs' \<subseteq> set2_iterm_pre v \<and> e' \<in> set3_iterm_pre v"
-  unfolding iLam_def iterm.TT_inject0
+lemma iLm_set3: "iterm_ctor v = iLm (xs::ivar dstream) e \<Longrightarrow>
+ \<exists>xs' e'. iterm_ctor v = iLm xs' e' \<and> dsset xs' \<subseteq> set2_iterm_pre v \<and> e' \<in> set3_iterm_pre v"
+  unfolding iLm_def iterm.TT_inject0
   apply (erule exE)
   apply (erule conjE)+
   subgoal for f
@@ -322,10 +321,10 @@ unfolding set2_iterm_pre_def set3_iterm_pre_def comp_def Abs_iterm_pre_inverse[O
   apply (rule conjI bij_imp_bij_inv supp_inv_bound singletonI | assumption)+
   by auto .
 
-lemma iLam_avoid: "|A::ivar set| <o |UNIV::ivar set| \<Longrightarrow> \<exists>xs' e'. iLam xs e = iLam xs' e' \<and> dsset xs' \<inter> A = {}"
-  apply (erule iterm.TT_fresh_cases[of _ "iLam xs e"])
+lemma iLm_avoid: "|A::ivar set| <o |UNIV::ivar set| \<Longrightarrow> \<exists>xs' e'. iLm xs e = iLm xs' e' \<and> dsset xs' \<inter> A = {}"
+  apply (erule iterm.TT_fresh_cases[of _ "iLm xs e"])
    apply (drule sym)
-  apply (frule iLam_set3)
+  apply (frule iLm_set3)
   apply (erule exE conjE)+
   apply (rule exI)+
   apply (rule conjI)
@@ -337,9 +336,9 @@ lemma iLam_avoid: "|A::ivar set| <o |UNIV::ivar set| \<Longrightarrow> \<exists>
   apply (drule iffD1[OF disjoint_iff])
   by auto
 
-lemma iLam_irrename:
+lemma iLm_irrename:
 "bij (\<sigma>::ivar\<Rightarrow>ivar) \<Longrightarrow> |supp \<sigma>| <o |UNIV:: ivar set| \<Longrightarrow>
- (\<And>a'. a' \<in> FFVars e - dsset (as::ivar dstream) \<Longrightarrow> \<sigma> a' = a') \<Longrightarrow> iLam as e = iLam (dsmap \<sigma> as) (irrename \<sigma> e)"
+ (\<And>a'. a' \<in> iFV e - dsset (as::ivar dstream) \<Longrightarrow> \<sigma> a' = a') \<Longrightarrow> iLm as e = iLm (dsmap \<sigma> as) (irrename \<sigma> e)"
 by (metis iterm.permute(3) iterm.permute_cong_id iterm.set(3))
 
 
@@ -359,7 +358,7 @@ corollary SSupp_upd_VVr_bound[simp,intro!]: "|SSupp (VVr(a:=(t::itrm)))| <o |UNI
   apply (rule iterm.SSupp_VVr_bound)
   done
 
-lemma SSupp_upd_iVar_bound[simp,intro!]: "|SSupp (iVar(a:=(t::itrm)))| <o |UNIV::ivar set|"
+lemma SSupp_upd_iVr_bound[simp,intro!]: "|SSupp (iVr(a:=(t::itrm)))| <o |UNIV::ivar set|"
 using SSupp_upd_VVr_bound by auto
 
 lemma SSupp_IImsupp_bound: "|SSupp \<sigma>| <o |UNIV:: ivar set| \<Longrightarrow> |IImsupp \<sigma>| <o |UNIV:: ivar set|"
@@ -427,24 +426,24 @@ using SSupp_irrename_bound[OF assms] unfolding o_def .
 
 (* *)
 lemma SSupp_update_irrename_bound:
-"|SSupp (iVar(\<sigma> (x::ivar) := irrename \<sigma> e))| <o |UNIV::ivar set|"
-using SSupp_upd_iVar_bound .
+"|SSupp (iVr(\<sigma> (x::ivar) := irrename \<sigma> e))| <o |UNIV::ivar set|"
+using SSupp_upd_iVr_bound .
 
 lemma IImsupp_irrename_update_su:
 assumes s[simp]: "bij (\<sigma>::ivar\<Rightarrow>ivar)" "|supp \<sigma>| <o |UNIV::ivar set|"
-shows "IImsupp (irrename \<sigma> \<circ> iVar(x := e)) \<subseteq>
-       imsupp \<sigma> \<union> {x} \<union> FVars_iterm e"
+shows "IImsupp (irrename \<sigma> \<circ> iVr(x := e)) \<subseteq>
+       imsupp \<sigma> \<union> {x} \<union> iFV e"
 unfolding IImsupp_def SSupp_def imsupp_def supp_def by (auto split: if_splits)
 
 lemma IImsupp_irrename_update_bound:
 assumes s[simp]: "bij (\<sigma>::ivar\<Rightarrow>ivar)" "|supp \<sigma>| <o |UNIV::ivar set|"
-shows "|IImsupp (irrename \<sigma> \<circ> iVar(x := e))| <o |UNIV::ivar set|"
+shows "|IImsupp (irrename \<sigma> \<circ> iVr(x := e))| <o |UNIV::ivar set|"
 using IImsupp_irrename_update_su[OF assms]
 by (meson Un_bound card_of_subset_bound imsupp_supp_bound infinite_ivar s(2) singl_bound iterm.set_bd_UNIV)
 
 lemma SSupp_irrename_update_bound:
 assumes s[simp]: "bij (\<sigma>::ivar\<Rightarrow>ivar)" "|supp \<sigma>| <o |UNIV::ivar set|"
-shows "|SSupp (irrename \<sigma> \<circ> iVar(x := e))| <o |UNIV::ivar set|"
+shows "|SSupp (irrename \<sigma> \<circ> iVr(x := e))| <o |UNIV::ivar set|"
 using IImsupp_irrename_update_bound[OF assms] unfolding IImsupp_def
 using SSupp_irrename_bound s(1) s(2) by auto
 
@@ -452,14 +451,14 @@ using SSupp_irrename_bound s(1) s(2) by auto
 
 lemmas infinite_UNIV[simp]
 
-lemma irrename_swap_Var1[simp]: "irrename (x \<leftrightarrow> xx) (iVar (x::ivar)) = iVar xx"
+lemma irrename_swap_Var1[simp]: "irrename (x \<leftrightarrow> xx) (iVr(x::ivar)) = iVr xx"
 apply(subst iterm.permute(1)) by auto
-lemma irrename_swap_Var2[simp]: "irrename (x \<leftrightarrow> xx) (iVar (xx::ivar)) = iVar x"
+lemma irrename_swap_Var2[simp]: "irrename (x \<leftrightarrow> xx) (iVr(xx::ivar)) = iVr x"
 apply(subst iterm.permute(1)) by auto
-lemma irrename_swap_Var3[simp]: "z \<notin> {x,xx} \<Longrightarrow> irrename (x \<leftrightarrow> xx) (iVar (z::ivar)) = iVar z"
+lemma irrename_swap_Var3[simp]: "z \<notin> {x,xx} \<Longrightarrow> irrename (x \<leftrightarrow> xx) (iVr(z::ivar)) = iVr z"
 apply(subst iterm.permute(1)) by auto
-lemma irrename_swap_Var[simp]: "irrename (x \<leftrightarrow> xx) (iVar (z::ivar)) =
- iVar (if z = x then xx else if z = xx then x else z)"
+lemma irrename_swap_Var[simp]: "irrename (x \<leftrightarrow> xx) (iVr(z::ivar)) =
+ iVr(if z = x then xx else if z = xx then x else z)"
 apply(subst iterm.permute(1)) by auto
 
 (* Compositionality properties of renaming and term-for-variable substitution *)
@@ -497,45 +496,45 @@ qed
 
 (* Unary (term-for-var) substitution versus renaming: *)
 
-lemma supp_SSupp_iVar_le[simp]: "SSupp (iVar \<circ> \<sigma>) = supp \<sigma>"
+lemma supp_SSupp_iVr_le[simp]: "SSupp (iVr\<circ> \<sigma>) = supp \<sigma>"
 unfolding supp_def SSupp_def by simp
 
-lemma irrename_eq_itvsubst_iVar:
+lemma irrename_eq_itvsubst_iVr:
 assumes "bij (\<sigma>::ivar\<Rightarrow>ivar)" "|supp \<sigma>| <o |UNIV::ivar set|"
-shows "irrename \<sigma> = itvsubst (iVar o \<sigma>)"
+shows "irrename \<sigma> = itvsubst (iVr o \<sigma>)"
 proof
   fix t
-  show "irrename \<sigma> t = itvsubst (iVar o \<sigma>) t"
-  proof (binder_induction t avoiding: "IImsupp (iVar \<circ> \<sigma>)" rule: iterm.strong_induct)
+  show "irrename \<sigma> t = itvsubst (iVr o \<sigma>) t"
+  proof (binder_induction t avoiding: "IImsupp (iVr\<circ> \<sigma>)" rule: iterm.strong_induct)
     case Bound
-    then show ?case using SSupp_IImsupp_bound assms by (metis supp_SSupp_iVar_le)
+    then show ?case using SSupp_IImsupp_bound assms by (metis supp_SSupp_iVr_le)
   next
-    case (iLam x1 x2)
+    case (iLm x1 x2)
     then show ?case using assms by (simp add: IImsupp_def disjoint_iff not_in_supp_alt dstream_map_ident_strong)
   qed (auto simp: assms intro: stream.map_cong)
 qed
 
-lemma irrename_eq_itvsubst_iVar':
-"bij (\<sigma>::ivar\<Rightarrow>ivar) \<Longrightarrow> |supp \<sigma>| <o |UNIV::ivar set| \<Longrightarrow> irrename \<sigma> e = itvsubst (iVar o \<sigma>) e"
-using irrename_eq_itvsubst_iVar by auto
+lemma irrename_eq_itvsubst_iVr':
+"bij (\<sigma>::ivar\<Rightarrow>ivar) \<Longrightarrow> |supp \<sigma>| <o |UNIV::ivar set| \<Longrightarrow> irrename \<sigma> e = itvsubst (iVr o \<sigma>) e"
+using irrename_eq_itvsubst_iVr by auto
 
 (* Equivariance of unary substitution: *)
 
 lemma itvsubst_irrename_comp[simp]:
 assumes s[simp]: "bij (\<sigma>::ivar\<Rightarrow>ivar)" "|supp \<sigma>| <o |UNIV::ivar set|"
-shows "itvsubst (irrename \<sigma> \<circ> iVar(x := e2)) e1 = itvsubst (iVar(\<sigma> x := irrename \<sigma> e2)) (irrename \<sigma> e1)"
+shows "itvsubst (irrename \<sigma> \<circ> iVr(x := e2)) e1 = itvsubst (iVr(\<sigma> x := irrename \<sigma> e2)) (irrename \<sigma> e1)"
 proof-
   note SSupp_irrename_update_bound[OF assms, unfolded comp_def, simplified, simp]
   note SSupp_update_irrename_bound[unfolded fun_upd_def, simplified, simp]
   show ?thesis
-  apply(induct e1 rule: iterm.fresh_induct[where A = "{x} \<union> FFVars e2 \<union> imsupp \<sigma>"])
+  apply(induct e1 rule: iterm.fresh_induct[where A = "{x} \<union> iFV e2 \<union> imsupp \<sigma>"])
     subgoal by (meson Un_bound imsupp_supp_bound infinite_ivar s(2) singl_bound iterm.set_bd_UNIV)
     subgoal by (auto simp: bij_implies_inject)
     subgoal apply simp by (smt (verit, best) comp_apply stream.map_comp stream.map_cong)
 
     subgoal for ys t apply simp apply(subgoal_tac
-      "dsset ys \<inter> IImsupp ((\<lambda>a. irrename \<sigma> (if a = x then e2 else iVar a))) = {} \<and>
-      \<sigma> ` dsset ys \<inter> IImsupp (\<lambda>a. if a = \<sigma> x then irrename \<sigma> e2 else iVar a) = {}")
+      "dsset ys \<inter> IImsupp ((\<lambda>a. irrename \<sigma> (if a = x then e2 else iVr a))) = {} \<and>
+      \<sigma> ` dsset ys \<inter> IImsupp (\<lambda>a. if a = \<sigma> x then irrename \<sigma> e2 else iVr a) = {}")
       subgoal
         by simp (metis (no_types, lifting) Int_Un_emptyI2 dstream_map_ident_strong imsupp_empty_IntD2)
       subgoal unfolding IImsupp_def imsupp_def SSupp_def supp_def by (auto split: if_splits simp: bij_implies_inject)  . .
@@ -543,18 +542,18 @@ qed
 
 (* Unary substitution versus swapping: *)
 lemma itvsubst_Var_irrename:
-assumes xx: "xx \<notin> FFVars e1 - {x}"
-shows "itvsubst (iVar((x::ivar) := e2)) e1 = itvsubst (iVar(xx := e2)) (irrename (x \<leftrightarrow> xx) e1)"
+assumes xx: "xx \<notin> iFV e1 - {x}"
+shows "itvsubst (iVr((x::ivar) := e2)) e1 = itvsubst (iVr(xx := e2)) (irrename (x \<leftrightarrow> xx) e1)"
 proof-
   show ?thesis using xx
-  apply(induct e1 rule: iterm.fresh_induct[where A = "{x,xx} \<union> FFVars e2"])
+  apply(induct e1 rule: iterm.fresh_induct[where A = "{x,xx} \<union> iFV e2"])
     subgoal by (metis insert_is_Un iterm.set_bd_UNIV singl_bound var_iterm_pre_class.Un_bound)
     subgoal by simp
     subgoal by simp (smt (verit, best) comp_apply stream.map_comp stream.map_cong)
     subgoal for ys t apply simp apply(subgoal_tac
-      "dsset ys \<inter> IImsupp (iVar(x := e2)) = {} \<and> dsset ys \<inter> IImsupp (iVar(xx := e2)) = {}")
+      "dsset ys \<inter> IImsupp (iVr(x := e2)) = {} \<and> dsset ys \<inter> IImsupp (iVr(xx := e2)) = {}")
       subgoal
-        by simp (metis SSupp_upd_iVar_bound dstream_map_ident_strong iterm.subst(3) swap_simps(3))
+        by simp (metis SSupp_upd_iVr_bound dstream_map_ident_strong iterm.subst(3) swap_simps(3))
       subgoal unfolding IImsupp_def imsupp_def SSupp_def supp_def by auto . .
 qed
 
@@ -570,7 +569,6 @@ lemma usub_swap_disj:
 assumes "{u,v} \<inter> {x,y} = {}"
 shows "usub (iswap t u v) x y = iswap (usub t x y) u v"
 proof-
-  note iterm.vvsubst_permute[simp del]
   show ?thesis using assms
   apply(subst iterm.vvsubst_permute[symmetric]) apply auto
   apply(subst iterm.map_comp) apply auto
@@ -589,15 +587,15 @@ by auto
 
 (* *)
 
-lemma iswap_simps[simp]: "iswap (iVar z) (y::ivar) x = iVar ((x \<leftrightarrow> y) z)"
-"iswap (iApp t ss) (y::ivar) x = iApp (iswap t y x) (smap (\<lambda>s. iswap s y x) ss)"
-"iswap (iLam vs t) (y::ivar) x = iLam (dsmap (y \<leftrightarrow> x) vs) (iswap t y x)"
+lemma iswap_simps[simp]: "iswap (iVr z) (y::ivar) x = iVr((x \<leftrightarrow> y) z)"
+"iswap (iAp t ss) (y::ivar) x = iAp (iswap t y x) (smap (\<lambda>s. iswap s y x) ss)"
+"iswap (iLm vs t) (y::ivar) x = iLm (dsmap (y \<leftrightarrow> x) vs) (iswap t y x)"
  by simp_all
 
-lemma FFVars_swap[simp]: "FFVars (iswap t y x) = (x \<leftrightarrow> y) ` (FFVars t)"
+lemma iFV_swap[simp]: "iFV (iswap t y x) = (x \<leftrightarrow> y) ` (iFV t)"
 apply(subst iterm.FVars_permute) by (auto simp: swap_sym)
 
-lemma FFVars_swap'[simp]: "{x::ivar,y} \<inter> FFVars t = {} \<Longrightarrow> iswap t x y = t"
+lemma iFV_swap'[simp]: "{x::ivar,y} \<inter> iFV t = {} \<Longrightarrow> iswap t x y = t"
 apply(rule iterm.permute_cong_id) apply auto by (metis swap_def)
 
 (* *)
@@ -644,14 +642,14 @@ proof-
   apply(auto simp: dsmap_alt) by (metis dsset_range range_eqI)
 qed
 
-lemma iLam_refresh':
+lemma iLm_refresh':
 "\<exists>f xs'. bij f \<and> |supp f| <o |UNIV::ivar set| \<and>
-      dsset xs' \<inter> dsset xs = {} \<and> dsset xs' \<inter> FFVars (iLam xs (t::itrm)) = {} \<and>
+      dsset xs' \<inter> dsset xs = {} \<and> dsset xs' \<inter> iFV (iLm xs (t::itrm)) = {} \<and>
       dsmap f xs = xs' \<and>
-      id_on (FFVars (iLam xs t)) f \<and>
-      iLam xs t = iLam xs' (irrename f t)"
+      id_on (iFV (iLm xs t)) f \<and>
+      iLm xs t = iLm xs' (irrename f t)"
 proof-
-  define V where "V = FFVars (iLam xs (t::itrm))"
+  define V where "V = iFV (iLm xs (t::itrm))"
   have V: "V \<inter> dsset xs = {}" "|V| <o |UNIV::ivar set|"
   unfolding V_def
     using iterm.set_bd_UNIV apply (auto simp: Int_commute)
@@ -670,13 +668,13 @@ proof-
     subgoal unfolding iterm.inject apply(rule exI[of _ f]) using f unfolding V_def by auto .
 qed
 
-lemma iLam_refresh:
+lemma iLm_refresh:
 "\<exists>f xs'. bij f \<and> |supp f| <o |UNIV::ivar set| \<and>
-      dsset xs' \<inter> dsset xs = {} \<and> dsset xs' \<inter> FFVars (t::itrm) = {} \<and>
+      dsset xs' \<inter> dsset xs = {} \<and> dsset xs' \<inter> iFV (t::itrm) = {} \<and>
       dsmap f xs = xs' \<and>
-      id_on (FFVars t - dsset xs) f \<and>
-      iLam xs t = iLam xs' (irrename f t)"
-using iLam_refresh'[of xs t]
+      id_on (iFV t - dsset xs) f \<and>
+      iLm xs t = iLm xs' (irrename f t)"
+using iLm_refresh'[of xs t]
 apply (elim exE conjE) subgoal for f xs' apply(intro exI[of _ f] exI[of _ xs'])
 apply(intro conjI)
   subgoal by simp
@@ -690,22 +688,22 @@ apply(intro conjI)
 
 (* *)
 
-lemma FFVars_usub[simp]: "FFVars (usub t y x) =
- (if x \<in> FFVars t then FFVars t - {x} \<union> {y} else FFVars t)"
+lemma iFV_usub[simp]: "iFV (usub t y x) =
+ (if x \<in> iFV t then iFV t - {x} \<union> {y} else iFV t)"
 apply(subst iterm.set_map) by auto
 
-lemma usub_simps_free[simp]: "\<And>y x. usub (iVar z) (y::ivar) x = iVar (sb z y x)"
-"\<And>y x t s. usub (iApp t ss) (y::ivar) x = iApp (usub t y x) (smap (\<lambda>s. usub s y x) ss)"
+lemma usub_simps_free[simp]: "\<And>y x. usub (iVr z) (y::ivar) x = iVr(sb z y x)"
+"\<And>y x t s. usub (iAp t ss) (y::ivar) x = iAp (usub t y x) (smap (\<lambda>s. usub s y x) ss)"
 by (auto simp: sb_def)
 
-lemma usub_iLam[simp]:
-"dsset vs \<inter> {x,y} = {} \<Longrightarrow> usub (iLam vs t) (y::ivar) x = iLam vs (usub t y x)"
+lemma usub_iLm[simp]:
+"dsset vs \<inter> {x,y} = {} \<Longrightarrow> usub (iLm vs t) (y::ivar) x = iLm vs (usub t y x)"
 apply(subst iterm.map)
   subgoal by auto
   subgoal by (auto simp: imsupp_def supp_def)
   subgoal by auto .
 
-lemmas usub_simps = usub_simps_free usub_iLam
+lemmas usub_simps = usub_simps_free usub_iLm
 
 (* *)
 
@@ -721,7 +719,7 @@ apply(induct t rule: iterm.fresh_induct[where A = "{x,u} \<union> supp \<sigma>"
   subgoal using assms by simp (meson le_UNIV_insert)
   subgoal by (auto simp: sb_def bij_implies_inject)
   subgoal using assms apply simp unfolding stream.map_comp apply(rule stream.map_cong0) by auto
-  subgoal using assms apply(subst usub_iLam) apply auto apply(subst usub_iLam) by (auto simp: bij_implies_inject) .
+  subgoal using assms apply(subst usub_iLm) apply auto apply(subst usub_iLm) by (auto simp: bij_implies_inject) .
 
 lemma sw_sb:
 "(z1 \<leftrightarrow> z2) (sb z u x) = sb ((z1 \<leftrightarrow> z2) z) ((z1 \<leftrightarrow> z2) u) ((z1 \<leftrightarrow> z2) x)"
@@ -743,7 +741,7 @@ apply(induct t rule: iterm.fresh_induct[where A = "{x,u,z1,z2}"])
       unfolding sw_sb by presburger . .
 
 lemma usub_refresh:
-assumes "xx \<notin> FFVars t \<or> xx = x"
+assumes "xx \<notin> iFV t \<or> xx = x"
 shows "usub t u x = usub (iswap t x xx) u xx"
 proof-
   show ?thesis using assms
@@ -774,12 +772,12 @@ apply(rule iterm.permute_cong)
 
 (* "making" the substitution function that maps each xs_i to es_i; only
 meaningful if xs is non-repetitive *)
-definition "imkSubst xs es \<equiv> \<lambda>x. if x \<in> dsset xs then snth es (dtheN xs x) else iVar x"
+definition "imkSubst xs es \<equiv> \<lambda>x. if x \<in> dsset xs then snth es (dtheN xs x) else iVr x"
 
 lemma imkSubst_dsnth[simp]: "imkSubst xs es (dsnth xs i) = snth es i"
 unfolding imkSubst_def using dsset_range by auto
 
-lemma imkSubst_idle[simp]: "\<not> x \<in> dsset xs \<Longrightarrow> imkSubst xs es x = iVar x"
+lemma imkSubst_idle[simp]: "\<not> x \<in> dsset xs \<Longrightarrow> imkSubst xs es x = iVr x"
 unfolding imkSubst_def by auto
 
 lemma card_dsset_ivar: "|dsset xs| <o |UNIV::ivar set|"
@@ -826,8 +824,8 @@ unfolding imkSubst_smap_irrename[OF assms, symmetric] using assms unfolding fun_
 
 lemma card_SSupp_itvsubst_imkSubst_irrename_inv:
 "bij (\<sigma>::ivar\<Rightarrow>ivar) \<Longrightarrow> |supp \<sigma>| <o |UNIV::ivar set| \<Longrightarrow>
- |SSupp (itvsubst (irrename \<sigma> \<circ> imkSubst xs es \<circ> inv \<sigma>) \<circ> (iVar \<circ> \<sigma>))| <o |UNIV::ivar set|"
-by (metis SSupp_itvsubst_bound SSupp_imkSubst imkSubst_smap_irrename_inv supp_SSupp_iVar_le)
+ |SSupp (itvsubst (irrename \<sigma> \<circ> imkSubst xs es \<circ> inv \<sigma>) \<circ> (iVr\<circ> \<sigma>))| <o |UNIV::ivar set|"
+by (metis SSupp_itvsubst_bound SSupp_imkSubst imkSubst_smap_irrename_inv supp_SSupp_iVr_le)
 
 lemma card_SSupp_imkSubst_irrename_inv:
 "bij (\<sigma>::ivar\<Rightarrow>ivar) \<Longrightarrow> |supp \<sigma>| <o |UNIV::ivar set|  \<Longrightarrow>
@@ -840,16 +838,16 @@ by (metis bij_betw_def bij_imp_bij_betw dsmap_alt dtheN imkSubst_dsnth)
 
 (* *)
 
-lemma iLam_inject_avoid:
+lemma iLm_inject_avoid:
 assumes X: "|X::ivar set| <o |UNIV::ivar set|" "X \<inter> dsset xs = {}" "X \<inter> dsset xs' = {}"
 shows
-"(iLam xs e = iLam xs' e') =
- (\<exists>f. bij f \<and> |supp f| <o |UNIV::ivar set| \<and> id_on (FFVars (iLam xs e)) f \<and> id_on X f \<and>
+"(iLm xs e = iLm xs' e') =
+ (\<exists>f. bij f \<and> |supp f| <o |UNIV::ivar set| \<and> id_on (iFV (iLm xs e)) f \<and> id_on X f \<and>
       dsmap f xs = xs' \<and> irrename f e = e')"
 proof
-  assume "iLam xs e = iLam xs' e'"
+  assume "iLm xs e = iLm xs' e'"
   then obtain f where
-  f: "bij f" "|supp f| <o |UNIV::ivar set|" "id_on (FFVars (iLam xs e)) f" "dsmap f xs = xs'" "irrename f e = e'"
+  f: "bij f" "|supp f| <o |UNIV::ivar set|" "id_on (iFV (iLm xs e)) f" "dsmap f xs = xs'" "irrename f e = e'"
   unfolding iterm.inject by auto
   have bf: "bij_betw f (dsset xs) (dsset xs')"
   using f unfolding bij_betw_def bij_def inj_on_def
@@ -858,7 +856,7 @@ proof
     by (meson card_dsset_ivar var_stream_class.Un_bound)
   have 1: "(dsset xs \<union> dsset xs') \<inter> X = {}"
     by (simp add: Int_commute assms(2) assms(3) boolean_algebra.conj_disj_distrib)
-  show "\<exists>f. bij f \<and> |supp f| <o |UNIV::ivar set| \<and> id_on (FFVars (iLam xs e)) f \<and> id_on X f \<and> dsmap f xs = xs' \<and> irrename f e = e'"
+  show "\<exists>f. bij f \<and> |supp f| <o |UNIV::ivar set| \<and> id_on (iFV (iLm xs e)) f \<and> id_on X f \<and> dsmap f xs = xs' \<and> irrename f e = e'"
   using ex_avoiding_bij[OF f(2,1) infinite_ivar iterm.set_bd_UNIV f(3) 0 1 X(1)]
   apply safe subgoal for g apply(rule exI[of _ g]) using X f unfolding imsupp_def supp_def id_on_def
   apply safe
@@ -878,13 +876,13 @@ qed(unfold iterm.inject, auto)
 
 (* *)
 
-lemma iLam_eq_imkSubst:
-assumes il: "iLam (xs::ivar dstream) e1 = iLam xs' e1'"
+lemma iLm_eq_imkSubst:
+assumes il: "iLm (xs::ivar dstream) e1 = iLm xs' e1'"
 shows "itvsubst (imkSubst xs es2) e1 = itvsubst (imkSubst xs' es2) e1'"
 proof-
-  obtain f where f: "bij f" "|supp f| <o |UNIV::ivar set|" "id_on (ILC.FFVars (iLam xs e1)) f"
+  obtain f where f: "bij f" "|supp f| <o |UNIV::ivar set|" "id_on (ILC.iFV (iLm xs e1)) f"
   and 0: "xs' = dsmap f xs" "e1' = irrename f e1" using il[unfolded iterm.inject] by auto
-  show ?thesis unfolding 0 apply(subst irrename_eq_itvsubst_iVar')
+  show ?thesis unfolding 0 apply(subst irrename_eq_itvsubst_iVr')
     subgoal by fact subgoal by fact
     subgoal apply(subst itvsubst_comp)
       subgoal by simp
@@ -901,16 +899,16 @@ qed
 
 (* RECURSOR PREPARATIONS: *)
 
-lemma iLam_inject_strong:
-assumes il: "iLam (xs::ivar dstream) e = iLam xs' e'"
+lemma iLm_inject_strong:
+assumes il: "iLm (xs::ivar dstream) e = iLm xs' e'"
 and ds: "dsset xs \<inter> dsset xs' = {}"
 shows "\<exists>f. bij f \<and> |supp f| <o |UNIV::ivar set| \<and>
-   id_on (- (dsset xs \<union> dsset xs')) f \<and> id_on (FFVars (iLam xs e)) f \<and>
+   id_on (- (dsset xs \<union> dsset xs')) f \<and> id_on (iFV (iLm xs e)) f \<and>
    id_on (dsset xs) (f o f) \<and>
    dsmap f xs = xs' \<and> irrename f e = e'"
 proof-
   obtain f where f: "bij f" "|supp f| <o |UNIV::ivar set|"  "dsmap f xs = xs'"
-  and ff: "id_on (FFVars (iLam xs e)) f" "irrename f e = e'"
+  and ff: "id_on (iFV (iLm xs e)) f" "irrename f e = e'"
   using assms unfolding iterm.inject by auto
   have bf: "bij_betw f (dsset xs) (dsset xs')"
   by (metis bij_imp_bij_betw dstream.set_map f)
@@ -938,20 +936,20 @@ proof-
       subgoal using f
         by (meson \<open>bij g\<close> \<open>|supp g| <o |UNIV|\<close> dstream.map_cong g_def)
       subgoal
-        by (metis \<open>bij g\<close> \<open>dsmap g xs = xs'\<close> \<open>id_on (FFVars (iLam xs e)) g\<close> \<open>|supp g| <o |UNIV|\<close> iLam_same_inject il iterm.inject(3) iterm.set(3)) .
+        by (metis \<open>bij g\<close> \<open>dsmap g xs = xs'\<close> \<open>id_on (iFV (iLm xs e)) g\<close> \<open>|supp g| <o |UNIV|\<close> iLm_same_inject il iterm.inject(3) iterm.set(3)) .
 qed
 
 
-lemma iLam_inject_strong':
-assumes il: "iLam (xs::ivar dstream) e = iLam xs' e'"
-and zs: "dsset zs \<inter> (dsset xs \<union> dsset xs' \<union> FFVars e \<union> FFVars e') = {}"
+lemma iLm_inject_strong':
+assumes il: "iLm (xs::ivar dstream) e = iLm xs' e'"
+and zs: "dsset zs \<inter> (dsset xs \<union> dsset xs' \<union> iFV e \<union> iFV e') = {}"
 shows
 "\<exists>f f'.
    bij f \<and> |supp f| <o |UNIV::ivar set| \<and>
-     id_on ((- (dsset xs \<union> dsset zs))) f \<and> id_on (FFVars (iLam xs e)) f \<and>
+     id_on ((- (dsset xs \<union> dsset zs))) f \<and> id_on (iFV (iLm xs e)) f \<and>
      id_on (dsset xs) (f o f) \<and> dsmap f xs = zs \<and>
    bij f' \<and> |supp f'| <o |UNIV::ivar set| \<and>
-     id_on (- (dsset xs' \<union> dsset zs)) f' \<and> id_on (FFVars (iLam xs' e')) f' \<and>
+     id_on (- (dsset xs' \<union> dsset zs)) f' \<and> id_on (iFV (iLm xs' e')) f' \<and>
      id_on (dsset xs') (f' o f') \<and> dsmap f' xs' = zs \<and>
    irrename f e = irrename f' e'"
 proof-
@@ -967,7 +965,7 @@ proof-
   have sg: "supp g \<subseteq> dsset xs \<union> dsset zs" unfolding g_def supp_def by auto
 
   have g: "bij g" "|supp g| <o |UNIV::ivar set|"
-   "id_on (- (dsset xs \<union> dsset zs)) g" "id_on (FFVars (iLam xs e)) g"
+   "id_on (- (dsset xs \<union> dsset zs)) g" "id_on (iFV (iLm xs e)) g"
    "id_on (dsset xs) (g o g)"
    "dsmap g xs = zs"
   subgoal unfolding bij_def apply(rule conjI)
@@ -1000,7 +998,7 @@ proof-
   have sg: "supp g' \<subseteq> dsset xs' \<union> dsset zs" unfolding g'_def supp_def by auto
 
   have g': "bij g'" "|supp g'| <o |UNIV::ivar set|"
-   "id_on (- (dsset xs' \<union> dsset zs)) g'" "id_on (FFVars (iLam xs' e')) g'"
+   "id_on (- (dsset xs' \<union> dsset zs)) g'" "id_on (iFV (iLm xs' e')) g'"
    "id_on (dsset xs') (g' o g')"
    "dsmap g' xs' = zs"
   subgoal unfolding bij_def apply(rule conjI)
@@ -1020,7 +1018,7 @@ proof-
    subgoal by (metis \<open>bij g'\<close> \<open>|supp g'| <o |UNIV|\<close> dstream.map_cong f'(1) f'(2) f'(3) g'_def) .
 
    obtain h where h: "bij h" "|supp h| <o |UNIV::ivar set|"
-   and hid: "id_on (FFVars (iLam xs e)) h" "dsmap h xs = xs'" and e': "e' = irrename h e"
+   and hid: "id_on (iFV (iLm xs e)) h" "dsmap h xs = xs'" and e': "e' = irrename h e"
    using il unfolding iterm.inject by auto
 
    have 000: "dsmap (g' o h) xs = dsmap g xs"
@@ -1046,22 +1044,22 @@ qed
 
 (* *)
 
-lemma itrm_irrename_induct[case_names iVar iApp iLam]:
-assumes iiVar: "\<And>x. P (iVar (x::ivar))"
-and iiApp: "\<And>e1 es2. P e1 \<Longrightarrow> (\<forall>e2\<in>sset es2. P e2) \<Longrightarrow> P (iApp e1 es2)"
-and iiLam: "\<And>xs e. (\<And>f. bij f \<Longrightarrow> |supp f| <o |UNIV::ivar set| \<Longrightarrow> P (irrename f e)) \<Longrightarrow> P (iLam xs e)"
+lemma itrm_irrename_induct[case_names iVr iAp iLm]:
+assumes iiVr: "\<And>x. P (iVr(x::ivar))"
+and iiAp: "\<And>e1 es2. P e1 \<Longrightarrow> (\<forall>e2\<in>sset es2. P e2) \<Longrightarrow> P (iAp e1 es2)"
+and iiLm: "\<And>xs e. (\<And>f. bij f \<Longrightarrow> |supp f| <o |UNIV::ivar set| \<Longrightarrow> P (irrename f e)) \<Longrightarrow> P (iLm xs e)"
 shows "P t"
 proof-
   have "\<forall>f. bij f \<and> |supp f| <o |UNIV::ivar set| \<longrightarrow> P (irrename f t)"
   proof(induct)
-    case (iVar x)
-    then show ?case using iiVar by auto
+    case (iVr x)
+    then show ?case using iiVr by auto
   next
-    case (iApp t1 t2)
-    then show ?case using iiApp by auto
+    case (iAp t1 t2)
+    then show ?case using iiAp by auto
   next
-    case (iLam xs t)
-    then show ?case using iiLam
+    case (iLm xs t)
+    then show ?case using iiLm
     by simp (metis bij_o iterm.permute_comp iterm_pre.supp_comp_bound)
   qed
   thus ?thesis apply(elim allE[of _ id]) by auto
@@ -1125,7 +1123,7 @@ lemma not_in_FVarsB_iLamB:
 "b \<in> B \<Longrightarrow> dsset xs \<inter> FVarsB (iLamB xs b) = {}"
 using FVarsB_iLamB by auto
 
-thm iLam_inject_strong
+thm iLm_inject_strong
 
 lemma iLamB_inject_strong_rev:
 assumes bb': "{b,b'} \<subseteq> B" and
@@ -1173,53 +1171,53 @@ and an even more general one if we replace it with iLamB_inject_strong'_rev.
 definition morFromTrm where
 "morFromTrm H \<equiv>
  (\<forall>e. H e \<in> B) \<and>
- (\<forall>x. H (iVar x) = iVarB x) \<and>
- (\<forall>e1 es2. H (iApp e1 es2) = iAppB (H e1) (smap H es2)) \<and>
- (\<forall>xs e. H (iLam xs e) = iLamB xs (H e)) \<and>
+ (\<forall>x. H (iVr x) = iVarB x) \<and>
+ (\<forall>e1 es2. H (iAp e1 es2) = iAppB (H e1) (smap H es2)) \<and>
+ (\<forall>xs e. H (iLm xs e) = iLamB xs (H e)) \<and>
  (\<forall>\<sigma> e. bij \<sigma> \<and> |supp \<sigma>| <o |UNIV::ivar set| \<longrightarrow> H (irrename \<sigma> e) = renB \<sigma> (H e)) \<and>
- (\<forall>e. FVarsB (H e) \<subseteq> FFVars e)"
+ (\<forall>e. FVarsB (H e) \<subseteq> iFV e)"
 
 (* *)
 
 inductive R where
-iVar: "R (iVar x) (iVarB x)"
+iVr: "R (iVr x) (iVarB x)"
 |
-iApp: "R e1 b1 \<Longrightarrow> stream_all2 R es2 bs2 \<Longrightarrow> R (iApp e1 es2) (iAppB b1 bs2)"
+iAp: "R e1 b1 \<Longrightarrow> stream_all2 R es2 bs2 \<Longrightarrow> R (iAp e1 es2) (iAppB b1 bs2)"
 |
-iLam: "R e b \<Longrightarrow> R (iLam xs e) (iLamB xs b)"
+iLm: "R e b \<Longrightarrow> R (iLm xs e) (iLamB xs b)"
 
 (* *)
 
-lemma R_iVar_elim[simp]: "R (iVar x) b \<longleftrightarrow> b = iVarB x"
+lemma R_iVr_elim[simp]: "R (iVr x) b \<longleftrightarrow> b = iVarB x"
 apply safe
   subgoal using R.cases by fastforce
   subgoal by (auto intro: R.intros) .
 
 lemma R_iApp_elim:
-assumes "R (iApp e1 es2) b"
+assumes "R (iAp e1 es2) b"
 shows "\<exists>b1 bs2. R e1 b1 \<and> stream_all2 R es2 bs2 \<and> b = iAppB b1 bs2"
-by (metis (no_types, lifting) R.cases assms iterm.inject iterm.distinct(3) iterm.distinct(6))
+by (metis (no_types, lifting) R.cases assms iterm.inject(2) iterm.distinct(3) iterm.distinct(6))
 
-lemma R_iLam_elim:
-assumes "R (iLam xs e) b"
-shows "\<exists>xs' e' b'. R e' b' \<and> iLam xs e = iLam xs' e' \<and> b = iLamB xs' b'"
+lemma R_iLm_elim:
+assumes "R (iLm xs e) b"
+shows "\<exists>xs' e' b'. R e' b' \<and> iLm xs e = iLm xs' e' \<and> b = iLamB xs' b'"
 using assms by (cases rule: R.cases) auto
 
 lemma R_total:
 "\<exists>b. R e b"
 proof(induct e)
-  case (iVar x)
+  case (iVr x)
   then show ?case by (auto intro: R.intros)
 next
-  case (iApp e1 es2)
+  case (iAp e1 es2)
   then obtain b1 where r1: "R e1 b1" by auto
-  from iApp obtain B where r2: "\<forall>e2 \<in> sset es2. R e2 (B e2)" by metis
+  from iAp obtain B where r2: "\<forall>e2 \<in> sset es2. R e2 (B e2)" by metis
   show ?case apply(rule exI[of _ "iAppB b1 (smap B es2)"])
-  apply(rule R.iApp)
+  apply(rule R.iAp)
     subgoal by fact
     subgoal by (simp add: r2 stream_all2_iff_snth) .
 next
-  case (iLam x1 e)
+  case (iLm x1 e)
   then show ?case by (auto intro: R.intros)
 qed
 
@@ -1229,25 +1227,25 @@ by simp_all (metis (no_types, lifting) iAppB_B stream_all2_iff_snth subsetI theN
 
 lemma R_main:
 "(\<forall>b b'. R e b \<longrightarrow> R e b' \<longrightarrow> b = b') \<and>
- (\<forall>b. R e b \<longrightarrow> FVarsB b \<subseteq> FFVars e) \<and>
+ (\<forall>b. R e b \<longrightarrow> FVarsB b \<subseteq> iFV e) \<and>
  (\<forall>b f. R e b \<and> bij f \<and> |supp f| <o |UNIV::ivar set|
         \<longrightarrow> R (irrename f e) (renB f b))"
 proof(induct e rule: itrm_irrename_induct)
-  case (iVar x)
+  case (iVr x)
   then show ?case using FVarsB_iVarB by auto
 next
-  case (iApp e1 es2)
-  note iApp11 = iApp(1)[THEN conjunct1, rule_format]
-  note iApp12 = iApp(1)[THEN conjunct2, THEN conjunct1, rule_format]
-  note iApp13 = iApp(1)[THEN conjunct2, THEN conjunct2, rule_format,
+  case (iAp e1 es2)
+  note iApp11 = iAp(1)[THEN conjunct1, rule_format]
+  note iApp12 = iAp(1)[THEN conjunct2, THEN conjunct1, rule_format]
+  note iApp13 = iAp(1)[THEN conjunct2, THEN conjunct2, rule_format,
      OF conjI, OF _ conjI]
-  note iApp21 = iApp(2)[rule_format, THEN conjunct1, rule_format]
-  note iApp22 = iApp(2)[rule_format, THEN conjunct2, THEN conjunct1, rule_format]
-  note iApp23 = iApp(2)[rule_format, THEN conjunct2, THEN conjunct2, rule_format,
+  note iApp21 = iAp(2)[rule_format, THEN conjunct1, rule_format]
+  note iApp22 = iAp(2)[rule_format, THEN conjunct2, THEN conjunct1, rule_format]
+  note iApp23 = iAp(2)[rule_format, THEN conjunct2, THEN conjunct2, rule_format,
      OF _ conjI, OF _ _ conjI]
 
   show ?case proof safe
-    fix b b' assume "R (iApp e1 es2) b" "R (iApp e1 es2) b'"
+    fix b b' assume "R (iAp e1 es2) b" "R (iAp e1 es2) b'"
     then obtain b1 bs2 b1' bs2' where R1: "R e1 b1" "R e1 b1'"
     and R2: "stream_all2 R es2 bs2" "stream_all2 R es2 bs2'"
     and b: "b = iAppB b1 bs2" "b' = iAppB b1' bs2'"
@@ -1258,7 +1256,7 @@ next
     unfolding stream_all2_iff_snth sset_range image_def stream_eq_nth by fastforce
     show "b = b'" unfolding b 1 2 ..
   next
-    fix b x assume "R (iApp e1 es2) b" and xx: "x \<in> FVarsB b"
+    fix b x assume "R (iAp e1 es2) b" and xx: "x \<in> FVarsB b"
     then obtain b1 bs2 where R1: "R e1 b1"
     and R2: "stream_all2 R es2 bs2"
     and b: "b = iAppB b1 bs2"
@@ -1271,15 +1269,15 @@ next
     have x: "x \<in> FVarsB b1 \<or> (\<exists>b2\<in>sset bs2. x \<in> FVarsB b2)"
     using xx b12 FVarsB_iAppB unfolding b by fastforce
 
-    have fb1: "FVarsB b1 \<subseteq> FFVars e1" using iApp12[OF R1] .
-    have fb2: "\<Union> (FVarsB ` (sset bs2)) \<subseteq> \<Union> (FFVars ` (sset es2))"
+    have fb1: "FVarsB b1 \<subseteq> iFV e1" using iApp12[OF R1] .
+    have fb2: "\<Union> (FVarsB ` (sset bs2)) \<subseteq> \<Union> (iFV ` (sset es2))"
     using iApp22 R2 unfolding stream_all2_iff_snth sset_range image_def by auto
 
-    show "x \<in> FFVars (iApp e1 es2)"
+    show "x \<in> iFV (iAp e1 es2)"
     using x fb1 fb2 by auto
   next
     fix b and f::"ivar \<Rightarrow> ivar"
-    assume "R (iApp e1 es2) b" and f: "bij f" "|supp f| <o |UNIV::ivar set|"
+    assume "R (iAp e1 es2) b" and f: "bij f" "|supp f| <o |UNIV::ivar set|"
     then obtain b1 bs2 where R1: "R e1 b1"
     and R2: "stream_all2 R es2 bs2" and b: "b = iAppB b1 bs2"
     using R_iApp_elim by blast
@@ -1288,51 +1286,51 @@ next
     using R1 R_B
     by auto (metis R2 R_B stream_all2_iff_snth theN)
 
-    have 0: "R (iApp (irrename f e1) (smap (irrename f) es2))
+    have 0: "R (iAp (irrename f e1) (smap (irrename f) es2))
             (iAppB (renB f b1) (smap (renB f) bs2))"
-    apply(rule R.iApp)
+    apply(rule R.iAp)
       subgoal using iApp13[OF R1 f] .
       subgoal using iApp23[OF _ _ f] R2
       unfolding stream_all2_iff_snth sset_range image_def by auto .
 
-    show "R (irrename f (iApp e1 es2)) (renB f b)"
+    show "R (irrename f (iAp e1 es2)) (renB f b)"
     unfolding b using 0
     using b12(1) b12(2) f(1) f(2) iterm.permute(2) renB_iAppB by auto
   qed
 next
-  case (iLam xs t)
-  note iLamm = iLam[rule_format]
+  case (iLm xs t)
+  note iLamm = iLm[rule_format]
   note iLam1 = iLamm[THEN conjunct1, rule_format]
   note iLam2 = iLamm[THEN conjunct2, THEN conjunct1, rule_format]
   note iLam3 = iLamm[THEN conjunct2, THEN conjunct2, rule_format, OF _ _ conjI, OF _ _ _ conjI]
   note iLam33 = iLam3[of id, simplified]
 
   show ?case proof safe
-    fix b1 b2 assume RiLam: "R (iLam xs t) b1" "R (iLam xs t) b2"
+    fix b1 b2 assume RiLm: "R (iLm xs t) b1" "R (iLm xs t) b2"
     then obtain xs1' t1' b1' xs2' t2' b2'
-    where 1: "R t1' b1'" "iLam xs t = iLam xs1' t1'" "b1 = iLamB xs1' b1'"
-    and   2: "R t2' b2'" "iLam xs t = iLam xs2' t2'" "b2 = iLamB xs2' b2'"
-    using R_iLam_elim by metis
+    where 1: "R t1' b1'" "iLm xs t = iLm xs1' t1'" "b1 = iLamB xs1' b1'"
+    and   2: "R t2' b2'" "iLm xs t = iLm xs2' t2'" "b2 = iLamB xs2' b2'"
+    using R_iLm_elim by metis
 
     have b12': "{b1',b2'} \<subseteq> B"
     using 1(1,3) 2(1,3) R_B by auto
 
-    have "|dsset xs \<union> dsset xs1' \<union> dsset xs2' \<union> FFVars t \<union> FFVars t1' \<union> FFVars t2'| <o |UNIV::ivar set|"
+    have "|dsset xs \<union> dsset xs1' \<union> dsset xs2' \<union> iFV t \<union> iFV t1' \<union> iFV t2'| <o |UNIV::ivar set|"
     by (meson card_dsset_ivar iterm.set_bd_UNIV var_stream_class.Un_bound)
     then obtain zs where zs:
-    "dsset zs \<inter> (dsset xs \<union> dsset xs1' \<union> dsset xs2' \<union> FFVars t \<union> FFVars t1' \<union> FFVars t2') = {}"
-    by (meson iLam_avoid)
+    "dsset zs \<inter> (dsset xs \<union> dsset xs1' \<union> dsset xs2' \<union> iFV t \<union> iFV t1' \<union> iFV t2') = {}"
+    by (meson iLm_avoid)
 
     obtain f1 f1' where
     f1: "bij f1" "|supp f1| <o |UNIV::ivar set|"
-       "id_on (- (dsset xs \<union> dsset zs)) f1 \<and> id_on (FFVars(iLam xs t)) f1"
+       "id_on (- (dsset xs \<union> dsset zs)) f1 \<and> id_on (iFV(iLm xs t)) f1"
        "id_on (dsset xs) (f1 o f1)" and
     f1': "bij f1'" "|supp f1'| <o |UNIV::ivar set|"
-       "id_on (- (dsset xs1' \<union> dsset zs)) f1' \<and> id_on (FFVars(iLam xs1' t1')) f1'"
+       "id_on (- (dsset xs1' \<union> dsset zs)) f1' \<and> id_on (iFV(iLm xs1' t1')) f1'"
        "id_on (dsset xs1') (f1' o f1')"
     and zs1: "dsmap f1 xs = zs" "dsmap f1' xs1' = zs"
     and f1f1': "irrename f1 t = irrename f1' t1'"
-    using zs iLam_inject_strong'[OF 1(2), of zs] by force
+    using zs iLm_inject_strong'[OF 1(2), of zs] by force
 
     have if1': "bij (inv f1' o f1)" "|supp (inv f1' o f1)| <o |UNIV::ivar set|"
     by (auto simp add: f1 f1' iterm_pre.supp_comp_bound)
@@ -1341,19 +1339,19 @@ next
     using f1f1' by (metis (mono_tags, lifting) bij_imp_bij_inv f1(1,2) f1'(1,2)
        inv_o_simp1 supp_inv_bound iterm.permute_comp iterm.permute_id)
 
-    have fvb1': "FVarsB b1' \<subseteq> FFVars t1'"
+    have fvb1': "FVarsB b1' \<subseteq> iFV t1'"
     using iLam2[OF if1', unfolded t1'[symmetric], OF 1(1)] .
 
     obtain f2 f2' where
     f2: "bij f2" "|supp f2| <o |UNIV::ivar set|"
-       "id_on (- (dsset xs \<union> dsset zs)) f2 \<and> id_on (FFVars(iLam xs t)) f2"
+       "id_on (- (dsset xs \<union> dsset zs)) f2 \<and> id_on (iFV(iLm xs t)) f2"
        "id_on (dsset xs) (f2 o f2)" and
     f2': "bij f2'" "|supp f2'| <o |UNIV::ivar set|"
-       "id_on (- (dsset xs2' \<union> dsset zs)) f2' \<and> id_on (FFVars(iLam xs2' t2')) f2'"
+       "id_on (- (dsset xs2' \<union> dsset zs)) f2' \<and> id_on (iFV(iLm xs2' t2')) f2'"
        "id_on (dsset xs2') (f2' o f2')"
     and zs2: "dsmap f2 xs = zs" "dsmap f2' xs2' = zs"
     and f2f2': "irrename f2 t = irrename f2' t2'"
-    using zs iLam_inject_strong'[OF 2(2), of zs] by force
+    using zs iLm_inject_strong'[OF 2(2), of zs] by force
 
     have if2': "bij (inv f2' o f2)" "|supp (inv f2' o f2)| <o |UNIV::ivar set|"
     by (auto simp add: f2 f2' iterm_pre.supp_comp_bound)
@@ -1363,7 +1361,7 @@ next
     by (metis (mono_tags, lifting) bij_imp_bij_inv f2(1,2) f2'(1,2)
       inv_o_simp1 iterm.permute_comp iterm.permute_id supp_inv_bound)
 
-    have fvb2': "FVarsB b2' \<subseteq> FFVars t2'"
+    have fvb2': "FVarsB b2' \<subseteq> iFV t2'"
     using iLam2[OF if2', unfolded t2'[symmetric], OF 2(1)] .
 
     have if2: "bij (inv f2)" "|supp (inv f2)| <o |UNIV::ivar set|"
@@ -1401,7 +1399,7 @@ next
     define ff2' where "ff2' = f1 o (inv f2) o f2'"
 
     have ff2': "bij ff2'" "|supp ff2'| <o |UNIV::ivar set|"
-       "id_on (- (dsset xs2' \<union> dsset zs)) ff2' \<and> id_on (FFVars (iLam xs2' t2')) ff2'"
+       "id_on (- (dsset xs2' \<union> dsset zs)) ff2' \<and> id_on (iFV (iLm xs2' t2')) ff2'"
     unfolding ff2'_def using f1 f2 f2'
       subgoal by auto
       subgoal unfolding ff2'_def using f1 f2 f2' by (simp add: iterm_pre.supp_comp_bound)
@@ -1438,10 +1436,10 @@ next
   (* *)
   next
     fix b y
-    assume R: "R (iLam xs t) b" and yy: "y \<in> FVarsB b"
+    assume R: "R (iLm xs t) b" and yy: "y \<in> FVarsB b"
     then obtain xs' t' b'
-    where 0: "R t' b'" "iLam xs t = iLam xs' t'" "b = iLamB xs' b'"
-    using R_iLam_elim by metis
+    where 0: "R t' b'" "iLm xs t = iLm xs' t'" "b = iLamB xs' b'"
+    using R_iLm_elim by metis
 
     have b': "b' \<in>  B"
     using 0(1,3) R_B by auto
@@ -1449,55 +1447,55 @@ next
     have y: "y \<notin> dsset xs'" "y \<in> FVarsB b'" using b' yy unfolding 0
     using FVarsB_iLamB[OF b'] by auto
 
-    have "|dsset xs \<union> dsset xs' \<union> FFVars t \<union> FFVars t'| <o |UNIV::ivar set|"
+    have "|dsset xs \<union> dsset xs' \<union> iFV t \<union> iFV t'| <o |UNIV::ivar set|"
     by (simp add: card_dsset_ivar iterm.set_bd_UNIV var_stream_class.Un_bound)
     then obtain z where z:
-    "z \<notin> dsset xs \<union> dsset xs' \<union> FFVars t \<union> FFVars t'"
+    "z \<notin> dsset xs \<union> dsset xs' \<union> iFV t \<union> iFV t'"
     by (meson exists_fresh)
 
     obtain f where
     f: "bij f" "|supp f| <o |UNIV::ivar set|"
-    "id_on (FFVars (iLam xs t)) f "
+    "id_on (iFV (iLm xs t)) f "
     and zs: "dsmap f xs = xs'"
     and t': "t' = irrename f t"
     using 0(2) unfolding iterm.inject by auto
 
-    have fvb't': "FVarsB b' \<subseteq> FFVars t'"
+    have fvb't': "FVarsB b' \<subseteq> iFV t'"
     using iLam2[OF f(1,2), unfolded t'[symmetric], OF 0(1)] .
-    have yt': "y \<in> FFVars t'" using fvb't' y(2) by auto
+    have yt': "y \<in> iFV t'" using fvb't' y(2) by auto
 
-    show "y \<in> FFVars(iLam xs t)" using yt' y unfolding 0(2) by auto
+    show "y \<in> iFV(iLm xs t)" using yt' y unfolding 0(2) by auto
 
   (* *)
   next
     fix b and f :: "ivar\<Rightarrow>ivar"
-    assume "R (iLam xs t) b" and f: "bij f" "|supp f| <o |UNIV::ivar set|"
+    assume "R (iLm xs t) b" and f: "bij f" "|supp f| <o |UNIV::ivar set|"
     then obtain xs' t' b'
-    where 0: "R t' b'" "iLam xs t = iLam xs' t'" "b = iLamB xs' b'"
-    using R_iLam_elim by metis
+    where 0: "R t' b'" "iLm xs t = iLm xs' t'" "b = iLamB xs' b'"
+    using R_iLm_elim by metis
 
     have b': "b' \<in>  B"
     using 0(1,3) R_B by auto
 
-    have "|dsset xs \<union> dsset xs' \<union> FFVars t \<union> FFVars t'| <o |UNIV::ivar set|"
+    have "|dsset xs \<union> dsset xs' \<union> iFV t \<union> iFV t'| <o |UNIV::ivar set|"
     by (meson card_dsset_ivar iterm.set_bd_UNIV var_stream_class.Un_bound)
 
     then obtain zs where zs:
-    "dsset zs \<inter> (dsset xs \<union> dsset xs' \<union> FFVars t \<union> FFVars t') = {}"
-    using iLam_avoid by blast
+    "dsset zs \<inter> (dsset xs \<union> dsset xs' \<union> iFV t \<union> iFV t') = {}"
+    using iLm_avoid by blast
 
-    obtain g where g: "bij g" "|supp g| <o |UNIV::ivar set|" "id_on (FFVars (iLam xs t)) g"
+    obtain g where g: "bij g" "|supp g| <o |UNIV::ivar set|" "id_on (iFV (iLm xs t)) g"
     and z: "dsmap g xs = xs'"
     and t': "t' = irrename g t"
     using 0(2) unfolding iterm.inject by auto
 
-    have RR: "R (iLam (dsmap f xs') (irrename f t')) (iLamB (dsmap f xs') (renB f b'))"
-    apply(rule R.iLam) unfolding t' apply(rule iLam3)
+    have RR: "R (iLm (dsmap f xs') (irrename f t')) (iLamB (dsmap f xs') (renB f b'))"
+    apply(rule R.iLm) unfolding t' apply(rule iLam3)
       subgoal by fact  subgoal by fact
       subgoal using 0(1) unfolding t' .
       subgoal by fact subgoal by fact .
 
-    show "R (irrename f (iLam xs t)) (renB f b)"
+    show "R (irrename f (iLm xs t)) (renB f b)"
     unfolding 0 using RR apply(subst iterm.permute)
       subgoal using f by auto subgoal using f by auto
       subgoal apply(subst renB_iLamB) using f b' by auto .
@@ -1505,7 +1503,7 @@ next
 qed
 
 lemmas R_functional = R_main[THEN conjunct1]
-lemmas R_FFVars= R_main[THEN conjunct2, THEN conjunct1]
+lemmas R_iFV= R_main[THEN conjunct2, THEN conjunct1]
 lemmas R_subst = R_main[THEN conjunct2, THEN conjunct2]
 
 (* *)
@@ -1518,12 +1516,12 @@ by (simp add: R_total H_def someI_ex)
 lemma ex_morFromTrm: "\<exists>H. morFromTrm H"
 apply(rule exI[of _ H]) unfolding morFromTrm_def apply(intro conjI)
   subgoal using R_B R_F by auto
-  subgoal using R.iVar R_F R_functional by blast
-  subgoal using R.iApp R_F R_functional unfolding stream_all2_iff_snth
+  subgoal using R.iVr R_F R_functional by blast
+  subgoal using R.iAp R_F R_functional unfolding stream_all2_iff_snth
     by (metis snth_smap)
-  subgoal using R.iLam R_F R_functional by blast
+  subgoal using R.iLm R_F R_functional by blast
   subgoal by (meson R_F R_functional R_subst)
-  subgoal by (simp add: R_F R_FFVars) .
+  subgoal by (simp add: R_F R_iFV) .
 
 definition rec where "rec \<equiv> SOME H. morFromTrm H"
 
@@ -1535,27 +1533,27 @@ by (metis ex_morFromTrm rec_def someI_ex)
 lemma rec_B[simp,intro!]: "rec e \<in> B"
 using morFromTrm_rec unfolding morFromTrm_def by auto
 
-lemma rec_iVar[simp]: "rec (iVar x) = iVarB x"
+lemma rec_iVr[simp]: "rec (iVr x) = iVarB x"
 using morFromTrm_rec unfolding morFromTrm_def by auto
 
-lemma rec_iApp[simp]: "rec (iApp e1 es2) = iAppB (rec e1) (smap rec es2)"
+lemma rec_iAp[simp]: "rec (iAp e1 es2) = iAppB (rec e1) (smap rec es2)"
 using morFromTrm_rec unfolding morFromTrm_def by auto
 
-lemma rec_iLam[simp]: "rec (iLam x e) = iLamB x (rec e)"
+lemma rec_iLm[simp]: "rec (iLm x e) = iLamB x (rec e)"
 using morFromTrm_rec unfolding morFromTrm_def by auto
 
 lemma rec_irrename: "bij \<sigma> \<Longrightarrow> |supp \<sigma>| <o |UNIV::ivar set| \<Longrightarrow>
  rec (irrename \<sigma> e) = renB \<sigma> (rec e)"
 using morFromTrm_rec unfolding morFromTrm_def by auto
 
-lemma FVarsB_rec: "FVarsB (rec e) \<subseteq> FFVars e"
+lemma FVarsB_rec: "FVarsB (rec e) \<subseteq> iFV e"
 using morFromTrm_rec unfolding morFromTrm_def by auto
 
 lemma rec_unique:
 assumes "\<And>e. H e \<in> B"
-"\<And>x. H (iVar x) = iVarB x"
-"\<And>e1 es2. H (iApp e1 es2) = iAppB (H e1) (smap H es2)"
-"\<And>xs e. H (iLam xs e) = iLamB xs (H e)"
+"\<And>x. H (iVr x) = iVarB x"
+"\<And>e1 es2. H (iAp e1 es2) = iAppB (H e1) (smap H es2)"
+"\<And>xs e. H (iLm xs e) = iLamB xs (H e)"
 shows "H = rec"
 apply(rule ext) subgoal for e apply(induct e)
 using assms by (auto cong: stream.map_cong) .
