thys/Infinitary_Lambda_Calculus/ILC_Head_Reduction.thy
@@ -5,7 +5,7 @@ begin
 (* Head reduction in the infinitary calculus: *)
 
 definition hred :: "ivar iterm \<Rightarrow> ivar iterm \<Rightarrow> bool" where 
-"hred e e' \<equiv> \<exists> xs e1 es2. e = iApp (iLam xs e1) es2 \<and> e' = itvsubst (imkSubst xs es2) e1"
+"hred e e' \<equiv> \<exists> xs e1 es2. e = iAp (iLm xs e1) es2 \<and> e' = itvsubst (imkSubst xs es2) e1"
 
 lemma hred_irrename: "bij \<sigma> \<Longrightarrow> |supp \<sigma>| <o |UNIV::ivar set| \<Longrightarrow> hred e e' \<Longrightarrow> hred (irrename \<sigma> e) (irrename \<sigma> e')"
 unfolding hred_def apply(elim exE) subgoal for xs e1 es2
@@ -14,7 +14,7 @@ unfolding hred_def apply(elim exE) subgoal for xs e1 es2
   apply(rule exI[of _ "smap (irrename \<sigma>) es2"])   
   apply (simp add: iterm.permute_comp) apply(subst irrename_itvsubst_comp) apply auto
   apply(subst imkSubst_smap_irrename_inv) unfolding isPerm_def apply auto 
-  apply(subst irrename_eq_itvsubst_iVar'[of _ e1]) unfolding isPerm_def apply auto
+  apply(subst irrename_eq_itvsubst_iVr'[of _ e1]) unfolding isPerm_def apply auto
   apply(subst itvsubst_comp) 
     subgoal by (metis SSupp_imkSubst imkSubst_smap_irrename_inv)
     subgoal by (smt (verit, best) SSupp_def VVr_eq_Var card_of_subset_bound mem_Collect_eq not_in_supp_alt o_apply subsetI) 
@@ -63,28 +63,28 @@ beta, which does not "hide" any freshness assumptions inside parameter predicate
 so its rule induction covers both beta and Xi. *)
 lemma hred_eq_avoid: 
 assumes A: "small A" and r: "hred e e'"
-shows "\<exists> xs e1 es2. dsset xs \<inter> \<Union> (FFVars ` (sset es2)) = {} \<and> dsset xs \<inter> A = {} \<and>
-            e = iApp (iLam xs e1) es2 \<and> e' = itvsubst (imkSubst xs es2) e1"
+shows "\<exists> xs e1 es2. dsset xs \<inter> \<Union> (iFV ` (sset es2)) = {} \<and> dsset xs \<inter> A = {} \<and>
+            e = iAp (iLm xs e1) es2 \<and> e' = itvsubst (imkSubst xs es2) e1"
 proof-
-  obtain xs e1 es2 where e: "e = iApp (iLam xs e1) es2" and e': "e' = itvsubst (imkSubst xs es2) e1" 
+  obtain xs e1 es2 where e: "e = iAp (iLm xs e1) es2" and e': "e' = itvsubst (imkSubst xs es2) e1" 
   using r unfolding hred_def by auto
-  define B where B: "B = A \<union> \<Union> (FFVars ` (sset es2))"
+  define B where B: "B = A \<union> \<Union> (iFV ` (sset es2))"
   have "small B" unfolding B
   apply(rule small_Un)
     subgoal by fact
     subgoal apply(rule small_UN)
       subgoal by (simp add: countable_card_ivar countable_sset)
       subgoal by (simp add: small_def iterm.set_bd_UNIV) . .
-  then obtain xs' e1' where 0: "iLam xs e1 = iLam xs' e1'" "dsset xs' \<inter> B = {}"
-  using iLam_avoid by (meson small_def)
+  then obtain xs' e1' where 0: "iLm xs e1 = iLm xs' e1'" "dsset xs' \<inter> B = {}"
+  using iLm_avoid by (meson small_def)
 
-  obtain f where f: "bij f" "|supp f| <o |UNIV::ivar set|" "id_on (FFVars (iLam xs e1)) f" 
+  obtain f where f: "bij f" "|supp f| <o |UNIV::ivar set|" "id_on (iFV (iLm xs e1)) f" 
   and 1: "xs' = dsmap f xs" "e1' = irrename f e1" using 0(1) unfolding iterm.inject by auto
   show ?thesis apply(intro exI[of _ xs'] exI[of _ e1'] exI[of _ es2]) apply(intro conjI)
     subgoal using 0(2) unfolding B by auto
     subgoal using 0(2) unfolding B by auto
     subgoal unfolding e 0(1) ..
-    subgoal unfolding e' 0(1) 1 apply(subst irrename_eq_itvsubst_iVar')
+    subgoal unfolding e' 0(1) 1 apply(subst irrename_eq_itvsubst_iVr')
       subgoal by fact  subgoal by fact
       subgoal apply(subst itvsubst_comp)
         subgoal by simp
@@ -95,13 +95,13 @@ proof-
           imkSubst_smap iterm.set(3)) . . 
 qed
 
-lemma hred_FFVars: "hred e e' \<Longrightarrow> FFVars e' \<subseteq> FFVars e"
+lemma hred_iFV: "hred e e' \<Longrightarrow> iFV e' \<subseteq> iFV e"
 unfolding hred_def by auto (metis imkSubst_def iterm.set(1) singletonD snth_sset)+
 
 lemma hred_determ: 
 "hred e e' \<Longrightarrow> hred e e'' \<Longrightarrow> e' = e''"
 unfolding hred_def  
-by auto (meson iLam_eq_imkSubst)
+by auto (meson iLm_eq_imkSubst)
 
 
 
