thys/Infinitary_Lambda_Calculus/ILC_affine.thy
@@ -7,19 +7,19 @@ begin
 
 (* *)
 
-lemma Tvars_dsset: "(FFVars t - dsset xs) \<inter> dsset xs = {}" "|FFVars t - dsset xs| <o |UNIV::ivar set|"
+lemma Tvars_dsset: "(iFV t - dsset xs) \<inter> dsset xs = {}" "|iFV t - dsset xs| <o |UNIV::ivar set|"
 apply auto using card_of_minus_bound iterm.set_bd_UNIV by blast
 
 inductive affine  :: "itrm \<Rightarrow> bool" where
- iVar[simp,intro!]: "affine (iVar x)"
-|iLam: "affine e \<Longrightarrow> affine (iLam xs e)"
-|iApp:
+ iVr[simp,intro!]: "affine (iVr x)"
+|iLm: "affine e \<Longrightarrow> affine (iLm xs e)"
+|iAp:
 "affine e1 \<Longrightarrow>
  (\<And>e2. e2 \<in> sset es2 \<Longrightarrow> affine e2) \<Longrightarrow>
- (\<And>e2. e2 \<in> sset es2 \<Longrightarrow> FFVars e1 \<inter> FFVars e2 = {}) \<Longrightarrow>
- (\<And>i j. i \<noteq> j \<Longrightarrow> FFVars (snth es2 i) \<inter> FFVars (snth es2 j) = {})
+ (\<And>e2. e2 \<in> sset es2 \<Longrightarrow> iFV e1 \<inter> iFV e2 = {}) \<Longrightarrow>
+ (\<And>i j. i \<noteq> j \<Longrightarrow> iFV (snth es2 i) \<inter> iFV (snth es2 j) = {})
  \<Longrightarrow>
- affine (iApp e1 es2)"
+ affine (iAp e1 es2)"
 
 binder_inductive affine
   subgoal premises prems for R B t
@@ -41,7 +41,7 @@ binder_inductive affine
           apply(rule exI[of _ "irrename f e"])
           apply(rule exI[of _ "dsmap f xs"])
           apply simp
-          subgoal apply(subst iLam_irrename[of "f"]) unfolding id_on_def by auto . . .
+          subgoal apply(subst iLm_irrename[of "f"]) unfolding id_on_def by auto . . .
         (* *)
     subgoal for e1 es2
       apply(rule exI[of _ "{}"])
@@ -56,95 +56,95 @@ binder_inductive affine
 thm affine.strong_induct
 thm affine.equiv
 
-(* ... and equivariance gives us a nice iLam inversion rule: *)
+(* ... and equivariance gives us a nice iLm inversion rule: *)
 
 lemma affine_App_case:
-"affine (iApp e1 es2) \<Longrightarrow>
+"affine (iAp e1 es2) \<Longrightarrow>
  affine e1 \<and>
- (\<forall>e2. e2 \<in> sset es2 \<longrightarrow> affine e2 \<and> FFVars e1 \<inter> FFVars e2 = {}) \<Longrightarrow>
- (\<forall>i j. i \<noteq> j \<longrightarrow> FFVars (snth es2 i) \<inter> FFVars (snth es2 j) = {})"
+ (\<forall>e2. e2 \<in> sset es2 \<longrightarrow> affine e2 \<and> iFV e1 \<inter> iFV e2 = {}) \<Longrightarrow>
+ (\<forall>i j. i \<noteq> j \<longrightarrow> iFV (snth es2 i) \<inter> iFV (snth es2 j) = {})"
 apply(subst (asm) affine.simps) by auto
 
 lemma affine_iApp_iff:
-"affine (iApp e1 es2) \<longleftrightarrow>
+"affine (iAp e1 es2) \<longleftrightarrow>
  (affine e1 \<and>
-  (\<forall>e2. e2 \<in> sset es2 \<longrightarrow> affine e2 \<and> FFVars e1 \<inter> FFVars e2 = {}) \<and>
-  (\<forall>i j. i \<noteq> j \<longrightarrow> FFVars (snth es2 i) \<inter> FFVars (snth es2 j) = {}))"
+  (\<forall>e2. e2 \<in> sset es2 \<longrightarrow> affine e2 \<and> iFV e1 \<inter> iFV e2 = {}) \<and>
+  (\<forall>i j. i \<noteq> j \<longrightarrow> iFV (snth es2 i) \<inter> iFV (snth es2 j) = {}))"
 apply(subst affine.simps) by auto
 
-lemma affine_iLam_case:
-assumes "affine (iLam xs e)"
+lemma affine_iLm_case:
+assumes "affine (iLm xs e)"
 shows "affine e"
 proof-
-  obtain xs' e' where 0: "iLam xs e = iLam xs' e'" and "affine e'"
+  obtain xs' e' where 0: "iLm xs e = iLm xs' e'" and "affine e'"
   using assms by (smt (verit, del_insts) affine.cases iterm.distinct(2) iterm.distinct(4))
   thus ?thesis using 0 unfolding iterm.inject
   by (metis iterm.inject(3) affine.equiv)
 qed
 
-lemma affine_iLam_iff[simp]:
-"affine (iLam xs e) \<longleftrightarrow> affine e"
-using affine.simps affine_iLam_case by blast
+lemma affine_iLm_iff[simp]:
+"affine (iLm xs e) \<longleftrightarrow> affine e"
+using affine.simps affine_iLm_case by blast
 
 (* Other properties: *)
 
 (* *)
 lemma tvsubst_affine':
 assumes f: "|SSupp f| <o |UNIV::ivar set|" and af: "\<And>x. affine (f x)"
-and fv: "\<And>x y. x \<noteq> y \<Longrightarrow> FFVars (f x) \<inter> FFVars (f y) = {}"
+and fv: "\<And>x y. x \<noteq> y \<Longrightarrow> iFV (f x) \<inter> iFV (f y) = {}"
 and r: "affine (e::itrm)"
 shows "affine (itvsubst f e)"
 using r proof (binder_induction e avoiding: "IImsupp f" rule: affine.strong_induct)
-  case (iLam ea xs)
-  show ?case using iLam apply(subst iterm.subst)
+  case (iLm ea xs)
+  show ?case using iLm apply(subst iterm.subst)
       subgoal using f by auto
       subgoal by auto
-      subgoal apply(rule affine.iLam) by auto .
+      subgoal apply(rule affine.iLm) by auto .
 next
-  case (iApp e1 es2)
+  case (iAp e1 es2)
   then show ?case apply(subst iterm.subst)
       subgoal using f by auto
-      subgoal apply(rule affine.iApp) using fv f
+      subgoal apply(rule affine.iAp) using fv f
       by auto (metis Int_emptyD)+ .
 qed (auto simp: f ILC.SSupp_IImsupp_bound af)
 
-(* Strengthening the previous result with "{x,y} \<subseteq> FFVars e "
+(* Strengthening the previous result with "{x,y} \<subseteq> iFV e "
 (which seems to prevent the above proof by induction), otherwise the result is
 not strong enough to instantiate to imakeSubst... *)
 lemma tvsubst_affine:
 assumes f: "|SSupp f| <o |UNIV::ivar set|" and af: "\<And>x. affine (f x)"
-and fv: "\<And>x y. {x,y} \<subseteq> FFVars e \<Longrightarrow> x \<noteq> y \<Longrightarrow> FFVars (f x) \<inter> FFVars (f y) = {}"
+and fv: "\<And>x y. {x,y} \<subseteq> iFV e \<Longrightarrow> x \<noteq> y \<Longrightarrow> iFV (f x) \<inter> iFV (f y) = {}"
 and r: "affine (e::itrm)"
 shows "affine (itvsubst f e)"
 proof-
   obtain xs and x::ivar where x: "x \<in> dsset xs"
     using dsset_range by blast
-  define t where "t = iLam xs (iVar x)"
-  have t: "FFVars t = {}" "affine t" unfolding t_def using x by (auto intro: affine.intros)
+  define t where "t = iLm xs (iVr x)"
+  have t: "iFV t = {}" "affine t" unfolding t_def using x by (auto intro: affine.intros)
 
-  have fve: "\<And>e. |FFVars e| <o |UNIV::ivar set|"
+  have fve: "\<And>e. |iFV e| <o |UNIV::ivar set|"
     by (simp add: iterm.set_bd_UNIV)
 
-  have "|\<Union> ((FFVars o f) ` (FFVars e))| \<le>o |Sigma (FFVars e) (FFVars o f)|"
+  have "|\<Union> ((iFV o f) ` (iFV e))| \<le>o |Sigma (iFV e) (iFV o f)|"
   by (rule card_of_UNION_Sigma)
-  also have "|Sigma (FFVars e) (FFVars o f)| <o |UNIV::ivar set|"
+  also have "|Sigma (iFV e) (iFV o f)| <o |UNIV::ivar set|"
   apply(rule stable_elim)
     subgoal by (metis exists_fresh UNIV_I card_ivar card_of_Field_ordIso card_of_nat
          finite_iff_ordLess_natLeq natLeq_Card_order ordIso_equivalence(3) ordIso_ordLess_trans
          ordLess_ordIso_trans stable_cardSuc stable_ordIso1)
     subgoal by fact
     subgoal unfolding o_def using fve . .
-  finally have ffv: "|\<Union> ((FFVars o f) ` (FFVars e))| <o |UNIV::ivar set|" .
+  finally have ffv: "|\<Union> ((iFV o f) ` (iFV e))| <o |UNIV::ivar set|" .
 
-  define g where "g \<equiv> \<lambda>x. if x \<in> FFVars e then f x
-                                           else if x \<in> \<Union> ((FFVars o f) ` (FFVars e)) then t
-                                           else iVar x"
-  have sg: "SSupp g \<subseteq> FFVars e \<union> \<Union> ((FFVars o f) ` (FFVars e))" unfolding g_def SSupp_def by auto
+  define g where "g \<equiv> \<lambda>x. if x \<in> iFV e then f x
+                                           else if x \<in> \<Union> ((iFV o f) ` (iFV e)) then t
+                                           else iVr x"
+  have sg: "SSupp g \<subseteq> iFV e \<union> \<Union> ((iFV o f) ` (iFV e))" unfolding g_def SSupp_def by auto
 
   have g: "|SSupp g| <o |UNIV::ivar set|" "\<And>x. affine (g x)"
-  "\<And>x y. x \<noteq> y \<Longrightarrow> FFVars (g x) \<inter> FFVars (g y) = {}"
+  "\<And>x y. x \<noteq> y \<Longrightarrow> iFV (g x) \<inter> iFV (g y) = {}"
      subgoal using sg by (meson card_of_subset_bound ffv fve var_stream_class.Un_bound)
-     subgoal by (simp add: af affine.iVar g_def t(2))
+     subgoal by (simp add: af g_def t(2))
      subgoal using fv unfolding g_def by (simp add: fv t(1)) .
 
   have 0: "itvsubst f e = itvsubst g e" apply(rule itvsubst_cong)
@@ -157,8 +157,8 @@ qed
 
 lemma imkSubst_affine:
 assumes r: "affine e" and
-fv: "\<And>e1. e1 \<in> sset es \<Longrightarrow> affine e1 \<and> FFVars e \<inter> FFVars e1 = {}"
-"\<And>i j. i \<noteq> j \<Longrightarrow> FFVars (snth es i) \<inter> FFVars (snth es j) = {}"
+fv: "\<And>e1. e1 \<in> sset es \<Longrightarrow> affine e1 \<and> iFV e \<inter> iFV e1 = {}"
+"\<And>i j. i \<noteq> j \<Longrightarrow> iFV (snth es i) \<inter> iFV (snth es j) = {}"
 shows "affine (itvsubst (imkSubst xs es) e)"
 apply(rule tvsubst_affine)
 using assms apply auto
@@ -167,8 +167,8 @@ using assms apply auto
 
 lemma imkSubst_affine_strong:
 assumes r: "affine e" and
-fv: "\<And>e1. e1 \<in> sset es \<Longrightarrow> affine e1 \<and> FFVars e \<inter> FFVars e1 \<subseteq> dsset xs"
-"\<And>i j. i \<noteq> j \<Longrightarrow> FFVars (snth es i) \<inter> FFVars (snth es j) = {}"
+fv: "\<And>e1. e1 \<in> sset es \<Longrightarrow> affine e1 \<and> iFV e \<inter> iFV e1 \<subseteq> dsset xs"
+"\<And>i j. i \<noteq> j \<Longrightarrow> iFV (snth es i) \<inter> iFV (snth es j) = {}"
 shows "affine (itvsubst (imkSubst xs es) e)"
 apply(rule tvsubst_affine)
 using assms apply auto
