thys/Infinitary_Lambda_Calculus/ILC_relations_more.thy
@@ -18,10 +18,10 @@ using assms proof (binder_induction e e' avoiding: e e' rule: istep.strong_induc
     unfolding affine_iApp_iff by fastforce+
 next
   case (iAppL e1 e1' es2)
-  then show ?case unfolding affine_iApp_iff using istep_FFVars by fastforce
+  then show ?case unfolding affine_iApp_iff using istep_iFV by fastforce
 next
   case (iAppR e1 es2 i e2')
-  then show ?case unfolding affine_iApp_iff using istep_FFVars
+  then show ?case unfolding affine_iApp_iff using istep_iFV
   by simp (smt (verit, ccfv_SIG) Int_subset_empty1 More_Stream.theN disjoint_iff snth_sset snth_supd_diff snth_supd_same)
 next
   case (Xi ea e'a xs)
@@ -37,13 +37,13 @@ using assms apply(induct rule: istep.induct)
     subgoal by (simp add: affine_iApp_iff) 
     subgoal using affine_iApp_iff by auto
     subgoal using affine_iApp_iff by auto .
-  subgoal unfolding affine_iApp_iff using istep_FFVars by fastforce
-    subgoal unfolding affine_iApp_iff using istep_FFVars 
+  subgoal unfolding affine_iApp_iff using istep_iFV by fastforce
+    subgoal unfolding affine_iApp_iff using istep_iFV 
     by simp (smt (verit, ccfv_SIG) Int_subset_empty1 More_Stream.theN disjoint_iff snth_sset snth_supd_diff snth_supd_same)
     subgoal by auto . 
 
 
-definition "affineS es \<equiv> (\<forall>e\<in>sset es. affine e) \<and> (\<forall>i j. i \<noteq> j \<longrightarrow> ILC.FFVars (snth es i) \<inter> ILC.FFVars (snth es j) = {})"
+definition "affineS es \<equiv> (\<forall>e\<in>sset es. affine e) \<and> (\<forall>i j. i \<noteq> j \<longrightarrow> ILC.iFV (snth es i) \<inter> ILC.iFV (snth es j) = {})"
 
 lemma hread_affine: "hred e e' \<Longrightarrow> affine e \<Longrightarrow> affine e'"
 using hred_def istep.Beta istep_affine by fastforce
@@ -51,12 +51,12 @@ using hred_def istep.Beta istep_affine by fastforce
 lemma hred_affineS: 
 "stream_all2 hred es es' \<Longrightarrow> affineS es \<Longrightarrow> affineS es'"
 using hread_affine unfolding stream_all2_iff_snth affineS_def sset_range 
-by auto (metis disjoint_iff_not_equal hred_def insert_absorb insert_subset istep.Beta istep_FFVars)
+by auto (metis disjoint_iff_not_equal hred_def insert_absorb insert_subset istep.Beta istep_iFV)
 
 
 lemma affineS_sflat: "affineS (sflat ess) \<longleftrightarrow> 
  (\<forall>i j i' j'. affine (snth2 ess (i,j)) \<and> 
-    ((i,j) \<noteq> (i',j') \<longrightarrow> ILC.FFVars ((snth2 ess (i,j))) \<inter> ILC.FFVars ((snth2 ess (i',j'))) = {}))"
+    ((i,j) \<noteq> (i',j') \<longrightarrow> ILC.iFV ((snth2 ess (i,j))) \<inter> ILC.iFV ((snth2 ess (i',j'))) = {}))"
 unfolding affineS_def sset_sflat sset_range image_def snth_sflat apply safe
   subgoal by (smt (verit, ccfv_threshold) UNIV_I mem_Collect_eq nat2_nat1 snth_sflat)
   subgoal apply auto by (metis Int_emptyD nat2_nat1 snth2.simps snth_sflat snth_supd_diff snth_supd_same)
@@ -66,9 +66,9 @@ unfolding affineS_def sset_sflat sset_range image_def snth_sflat apply safe
 
 
 lemma affineS_smap2_iApp_iff: 
-"affineS (smap2 iApp es ess) \<longleftrightarrow> 
+"affineS (smap2 iAp es ess) \<longleftrightarrow> 
  affineS es \<and> affineS (sflat ess) \<and> 
-  (\<forall>i j k. ILC.FFVars (snth es i) \<inter> ILC.FFVars (snth2 ess (j,k)) = {})"
+  (\<forall>i j k. ILC.iFV (snth es i) \<inter> ILC.iFV (snth2 ess (j,k)) = {})"
 unfolding affineS_def sset_sflat sset_range image_def snth_sflat affineS_sflat Un_def Int_def apply safe
   subgoal using affine_iApp_iff by fastforce
   subgoal by auto
@@ -85,8 +85,8 @@ unfolding affineS_def sset_sflat sset_range image_def snth_sflat affineS_sflat U
     by (smt (verit, ccfv_SIG) More_Stream.theN nat2_nat1 prod.inject snth2.simps) .
 
 
-lemma affineS_smap_iLam_iff: "affineS (smap (iLam xs) es) \<longleftrightarrow> 
-  (\<forall>i j. i \<noteq> j \<longrightarrow> affine (snth es i) \<and> ILC.FFVars (snth es i) \<inter> ILC.FFVars (snth es j) \<subseteq> dsset xs)"
+lemma affineS_smap_iLm_iff: "affineS (smap (iLm xs) es) \<longleftrightarrow> 
+  (\<forall>i j. i \<noteq> j \<longrightarrow> affine (snth es i) \<and> ILC.iFV (snth es i) \<inter> ILC.iFV (snth es j) \<subseteq> dsset xs)"
 unfolding affineS_def by auto (metis More_Stream.theN nat.simps(3))
 
 (* *)
@@ -96,18 +96,18 @@ assumes "ustepD d es es'"
 shows "\<forall>i. affine (es !! i) \<longrightarrow> affine (es' !! i)"
 using assms apply(induct rule: ustepD.induct)
   subgoal for es es' unfolding stream_all2_iff_snth using hread_affine by auto
-  subgoal apply auto unfolding affine_iApp_iff using ustepD_FFVars by fastforce
-  subgoal apply auto unfolding affine_iApp_iff using ustepD_FFVars 
+  subgoal apply auto unfolding affine_iApp_iff using ustepD_iFV by fastforce
+  subgoal apply auto unfolding affine_iApp_iff using ustepD_iFV 
   apply (auto simp: snth_sflat sset_range image_def)
     apply (metis nat2_nat1 snth2.simps) 
     apply (metis Int_emptyD in_mono nat2_nat1 snth2.simps snth_sflat)
     by (metis Int_emptyD insert_absorb insert_subset nat2_nat1 snth2.simps snth_sflat) 
-  subgoal for es es' xs apply(frule ustepD_FFVars) by auto  . 
+  subgoal for es es' xs apply(frule ustepD_iFV) by auto  . 
 
 lemma ustepD_affineS:
 assumes "ustepD d es es'" and "affineS es"
 shows "affineS es'"
-using assms ustepD_affine ustepD_FFVars unfolding affineS_def apply auto 
+using assms ustepD_affine ustepD_iFV unfolding affineS_def apply auto 
   apply (metis More_Stream.theN snth_sset)
   by (meson disjoint_iff_not_equal in_mono)
 
