thys/Infinitary_Lambda_Calculus/ILC_uniform.thy
@@ -24,49 +24,49 @@ will require (1) the custom presSuper equivariance and (2) a custom supervariabl
 lambda.  *)
 
 
-lemma reneqv_iVar_casesL:
-"reneqv (iVar x) e' \<Longrightarrow> 
- (\<exists> xs x'. e' = iVar x' \<and> super xs \<and> {x,x'} \<subseteq> dsset xs)"
+lemma reneqv_iVr_casesL:
+"reneqv (iVr x) e' \<Longrightarrow> 
+ (\<exists> xs x'. e' = iVr x' \<and> super xs \<and> {x,x'} \<subseteq> dsset xs)"
 apply(erule reneqv.cases) by auto
 
-lemma reneqv_iVar_casesR:
-"reneqv e (iVar x') \<Longrightarrow> 
- (\<exists> xs x. e = iVar x \<and> super xs \<and> {x,x'} \<subseteq> dsset xs)"
+lemma reneqv_iVr_casesR:
+"reneqv e (iVr x') \<Longrightarrow> 
+ (\<exists> xs x. e = iVr x \<and> super xs \<and> {x,x'} \<subseteq> dsset xs)"
 apply(erule reneqv.cases) by auto
 
 
 
-lemma uniform_iLam_inject_super: 
-assumes u: "uniform (iLam xs e)" and eq: "iLam xs e = iLam xs' e'" and super: "super xs" "super xs'"
+lemma uniform_iLm_inject_super: 
+assumes u: "uniform (iLm xs e)" and eq: "iLm xs e = iLm xs' e'" and super: "super xs" "super xs'"
 shows "\<exists>f. bij f \<and> |supp f| <o |UNIV::ivar set| \<and> presSuper f \<and> finite (touchedSuper (supp f)) \<and>
-       id_on (ILC.FFVars (iLam xs e)) f \<and> id_on (- (dsset xs \<union> dsset xs')) f \<and> 
+       id_on (ILC.iFV (iLm xs e)) f \<and> id_on (- (dsset xs \<union> dsset xs')) f \<and> 
        id_on (dsset xs) (f o f) \<and> dsmap f xs = xs' \<and> irrename f e = e'"
-apply(rule iLam_inject_super) using assms  
-by (metis finite_Diff2 finite_singleton touchedSuper_iLam uniform_finite_touchedUponT, auto)
+apply(rule iLm_inject_super) using assms  
+by (metis finite_Diff2 finite_singleton touchedSuper_iLm uniform_finite_touchedUponT, auto)
 
 
-lemma reneqv_iLam_casesL:
-assumes xs: "super xs" and rr: "reneqv (iLam xs e) ee'"
-shows "\<exists> e'. ee' = iLam xs e' \<and> reneqv e e'"
+lemma reneqv_iLm_casesL:
+assumes xs: "super xs" and rr: "reneqv (iLm xs e) ee'"
+shows "\<exists> e'. ee' = iLm xs e' \<and> reneqv e e'"
 proof-
-  obtain xsa ea ea' where il: "iLam xs e = iLam xsa ea" and ee': "ee' = iLam xsa ea'" 
+  obtain xsa ea ea' where il: "iLm xs e = iLm xsa ea" and ee': "ee' = iLm xsa ea'" 
   and xsa: "super xsa" and r: "reneqv ea ea'" 
   using rr by cases auto
 
-  have u: "uniform (iLam xsa ea)" using rr unfolding uniform_def ee' il by auto
+  have u: "uniform (iLm xsa ea)" using rr unfolding uniform_def ee' il by auto
   
   obtain f where f: "bij f" "|supp f| <o |UNIV::ivar set|" "presSuper f" 
-  "id_on (FFVars (iLam xsa ea)) f" "id_on (- (dsset xsa \<union> dsset xs)) f" 
+  "id_on (iFV (iLm xsa ea)) f" "id_on (- (dsset xsa \<union> dsset xs)) f" 
   and xsaa: "dsmap f xsa = xs" and e: "e = irrename f ea"
-  using uniform_iLam_inject_super[OF u il[symmetric] xsa xs] by auto
+  using uniform_iLm_inject_super[OF u il[symmetric] xsa xs] by auto
 
   have ff: "f ` (dsset xsa) = dsset xs" by (simp add: f(1) f(2) xsaa[symmetric])
 
-  have "FFVars (iLam xs e) \<inter> dsset xs = {}" by auto
-  hence "FFVars ee' \<inter> dsset xs = {}"  
+  have "iFV (iLm xs e) \<inter> dsset xs = {}" by auto
+  hence "iFV ee' \<inter> dsset xs = {}"  
   using reneqv_touchedSuperT_eq[OF rr] xs unfolding touchedSuperT_def touchedSuper_def by auto
-  hence "FFVars ea' \<inter> dsset xs \<subseteq> dsset xsa" unfolding ee' by auto
-  hence fv: "FFVars ea' \<inter> dsset xs = {} \<or> xs = xsa"  
+  hence "iFV ea' \<inter> dsset xs \<subseteq> dsset xsa" unfolding ee' by auto
+  hence fv: "iFV ea' \<inter> dsset xs = {} \<or> xs = xsa"  
   using super_disj[OF xs xsa] by auto
 
   show ?thesis apply(rule exI[of _ "irrename f ea'"]) apply(intro conjI)
@@ -79,30 +79,30 @@ proof-
     subgoal unfolding e using f(1) f(2) f(3) r irrename_reneqv by blast . 
 qed
 
-lemma reneqv_iLam_casesR:
-assumes xs: "super xs'" and rr: "reneqv ee (iLam xs' e')"
-shows "\<exists> e. ee = iLam xs' e \<and> reneqv e e'"
-using reneqv_iLam_casesL reneqv_sym rr xs by blast
+lemma reneqv_iLm_casesR:
+assumes xs: "super xs'" and rr: "reneqv ee (iLm xs' e')"
+shows "\<exists> e. ee = iLm xs' e \<and> reneqv e e'"
+using reneqv_iLm_casesL reneqv_sym rr xs by blast
 
-lemma reneqv_iLam_iff:
+lemma reneqv_iLm_iff:
 assumes "super xs"
-shows "reneqv (iLam xs e) (iLam xs e') \<longleftrightarrow> reneqv e e'"
-by (metis assms iLam_same_inject reneqv.iLam reneqv_iLam_casesR)
+shows "reneqv (iLm xs e) (iLm xs e') \<longleftrightarrow> reneqv e e'"
+by (metis assms iLm_same_inject reneqv.iLm reneqv_iLm_casesR)
 
 lemma reneqv_iApp_casesL:
-assumes rr: "reneqv (iApp e1 es2) ee'"
-shows "\<exists> e1' es2'. ee' = iApp e1' es2' \<and> reneqv e1 e1' \<and> 
+assumes rr: "reneqv (iAp e1 es2) ee'"
+shows "\<exists> e1' es2'. ee' = iAp e1' es2' \<and> reneqv e1 e1' \<and> 
           (\<forall>e e'. {e,e'} \<subseteq> sset es2 \<union> sset es2' \<longrightarrow> reneqv e e')"
 using assms by cases auto
 
 lemma reneqv_iApp_casesR:
-assumes rr: "reneqv ee (iApp e1' es2')"
-shows "\<exists> e1 es2. ee = iApp e1 es2 \<and> reneqv e1 e1' \<and> 
+assumes rr: "reneqv ee (iAp e1' es2')"
+shows "\<exists> e1 es2. ee = iAp e1 es2 \<and> reneqv e1 e1' \<and> 
           (\<forall>e e'. {e,e'} \<subseteq> sset es2 \<union> sset es2' \<longrightarrow> reneqv e e')"
 using assms by cases auto
 
 lemma reneqv_iApp_iff:
-"reneqv (iApp e1 es2) (iApp e1' es2') \<longleftrightarrow> 
+"reneqv (iAp e1 es2) (iAp e1' es2') \<longleftrightarrow> 
  reneqv e1 e1' \<and> (\<forall>e e'. {e,e'} \<subseteq> sset es2 \<union> sset es2' \<longrightarrow> reneqv e e')"
 apply(subst reneqv.simps) by auto
 
@@ -110,21 +110,21 @@ apply(subst reneqv.simps) by auto
 lemma reneqv_trans:
 "reneqv e e' \<Longrightarrow> reneqv e' e'' \<Longrightarrow> reneqv e e''"
 proof(induct arbitrary: e'' rule: reneqv.induct)
-  case (iVar xs x x')
-  then show ?case using reneqv_iVar_casesL[OF iVar(3)]
-  using super_disj by (auto intro!: reneqv.iVar) 
+  case (iVr xs x x')
+  then show ?case using reneqv_iVr_casesL[OF iVr(3)]
+  using super_disj by (auto intro!: reneqv.iVr) 
 next
-  case (iLam xs e e')
-  then show ?case using reneqv.iLam reneqv_iLam_casesL by blast
+  case (iLm xs e e')
+  then show ?case using reneqv.iLm reneqv_iLm_casesL by blast
 next
-  case (iApp e1 e1' es2 es2')
-  obtain e1'' es2'' where e'': "e'' = iApp e1'' es2''" 
+  case (iAp e1 e1' es2 es2')
+  obtain e1'' es2'' where e'': "e'' = iAp e1'' es2''" 
   and 1: "reneqv e1' e1''" 
   and 2: "(\<forall>e e'. {e, e'} \<subseteq> sset es2' \<union> sset es2'' \<longrightarrow> reneqv e e')"
-  using reneqv_iApp_casesL[OF iApp(4)] by auto
-  show ?case unfolding e'' apply(rule reneqv.iApp)
-    subgoal using iApp.hyps(2) 1 by blast
-    subgoal using iApp.hyps(3) 2  
+  using reneqv_iApp_casesL[OF iAp(4)] by auto
+  show ?case unfolding e'' apply(rule reneqv.iAp)
+    subgoal using iAp.hyps(2) 1 by blast
+    subgoal using iAp.hyps(3) 2  
     by auto (meson reneqv_sym snth_sset)+ .
 qed 
 
@@ -156,25 +156,25 @@ next
   case Bound2
   then show ?case using s ILC.SSupp_IImsupp_bound by auto
 next
-  case (iVar xs x x')
+  case (iVr xs x x')
   then show ?case using s rr by auto
 next
-  case (iLam ea e'a xs)
-  then show ?case using iLam apply(subst iterm.subst)
+  case (iLm ea e'a xs)
+  then show ?case using iLm apply(subst iterm.subst)
     subgoal using s by auto
     subgoal using s by auto
     apply(subst iterm.subst)
     subgoal using s by auto
     subgoal using s by auto
-    subgoal apply(rule reneqv.iLam) by auto .
+    subgoal apply(rule reneqv.iLm) by auto .
 next
-  case (iApp e1 e1' es2 es2')
+  case (iAp e1 e1' es2 es2')
   then show ?case using rr
     apply(subst iterm.subst)
     subgoal using s by auto
     apply(subst iterm.subst)
     subgoal using s by auto
-    subgoal apply(rule reneqv.iApp) apply auto
+    subgoal apply(rule reneqv.iAp) apply auto
       by (meson reneqv_trans reneqv_sym)+ .
 qed
 
@@ -204,18 +204,18 @@ lemma uniformS_def4:
 using uniformS_def3[unfolded reneqvS_def] .
 
 lemma uniformS_smap2_iApp_iff: 
-"uniformS (smap2 iApp es ess) \<longleftrightarrow> uniformS es \<and> uniformS (sflat ess)"
+"uniformS (smap2 iAp es ess) \<longleftrightarrow> uniformS es \<and> uniformS (sflat ess)"
 unfolding uniformS_def4 sset_sflat sset_smap2 unfolding sset_range apply auto
-  apply (metis iterm.inject reneqv_iApp_casesR)
-  subgoal for i j i' j' apply(erule allE[of _ "iApp (es !! i) (ess !! i)"])
-  apply(erule allE[of _ "iApp (es !! i') (ess !! i')"]) apply auto
+  apply (metis iterm.inject(2) reneqv_iApp_casesR)
+  subgoal for i j i' j' apply(erule allE[of _ "iAp (es !! i) (ess !! i)"])
+  apply(erule allE[of _ "iAp (es !! i') (ess !! i')"]) apply auto
   using reneqv_iApp_casesR by fastforce
-  subgoal by (metis Un_iff insert_subset rangeI reneqv.iApp sset_range) .
+  subgoal by (metis Un_iff insert_subset rangeI reneqv.iAp sset_range) .
 
-lemma uniformS_smap2_iLam_iff:
+lemma uniformS_smap2_iLm_iff:
 assumes "super xs"
-shows "uniformS (smap (iLam xs) es) \<longleftrightarrow> uniformS es"
-using assms unfolding uniformS_def4 by (force simp: image_def reneqv_iLam_iff) 
+shows "uniformS (smap (iLm xs) es) \<longleftrightarrow> uniformS es"
+using assms unfolding uniformS_def4 by (force simp: image_def reneqv_iLm_iff) 
 
 lemma uniformS_sset_uniform: "uniformS es \<Longrightarrow> e \<in> sset es \<Longrightarrow> uniform e"
 using reneqvS_def uniformS_def2 uniform_def3 by auto
@@ -225,11 +225,11 @@ lemma uniformS_touchedSuperT_eq:
 using reneqvS_def reneqv_touchedSuperT_eq uniformS_def3 by auto
 
 lemma uniformS_touchedSuper_eq: 
-"uniformS es \<Longrightarrow> {e,e'} \<subseteq> sset es \<Longrightarrow> touchedSuper (FFVars e) = touchedSuper (FFVars e')"
+"uniformS es \<Longrightarrow> {e,e'} \<subseteq> sset es \<Longrightarrow> touchedSuper (iFV e) = touchedSuper (iFV e')"
 using uniformS_touchedSuperT_eq touchedSuperT_def by auto
 
 lemma uniformS_touchedSuper: 
-"uniformS es \<Longrightarrow> e \<in> sset es \<Longrightarrow> touchedSuper (\<Union> (FFVars ` (sset es))) = touchedSuper (FFVars e)"
+"uniformS es \<Longrightarrow> e \<in> sset es \<Longrightarrow> touchedSuper (\<Union> (iFV ` (sset es))) = touchedSuper (iFV e)"
 unfolding touchedSuper_UN  
 by auto (metis empty_subsetI insert_subset touchedSuperT_def uniformS_touchedSuperT_eq) 
 
@@ -237,18 +237,18 @@ by auto (metis empty_subsetI insert_subset touchedSuperT_def uniformS_touchedSup
 
 lemma uniformS_touchedSuper_IImsupp_imkSubst: 
 "super xs \<Longrightarrow> uniformS es \<Longrightarrow> e \<in> sset es \<Longrightarrow> touchedSuper (IImsupp (imkSubst xs es)) \<subseteq> 
- {xs} \<union> touchedSuper (FFVars e)"
+ {xs} \<union> touchedSuper (iFV e)"
 using touchedSuper_IImsupp_imkSubst uniformS_touchedSuper by blast
 
 lemma uniformS_touchedSuper_IImsupp_imkSubst':
 "super xs \<Longrightarrow> uniformS es \<Longrightarrow> e \<in> sset es \<Longrightarrow> 
-  ys \<noteq> xs \<Longrightarrow> ys \<notin> touchedSuper (ILC.FFVars e) \<Longrightarrow> 
+  ys \<noteq> xs \<Longrightarrow> ys \<notin> touchedSuper (ILC.iFV e) \<Longrightarrow> 
   ys \<notin> touchedSuper (ILC.IImsupp (imkSubst xs es))"
 using uniformS_touchedSuper_IImsupp_imkSubst by auto
 
 lemma uniformS_touchedSuper_IImsupp_imkSubst'':
 "super xs \<Longrightarrow> super ys \<Longrightarrow> uniformS es \<Longrightarrow> e \<in> sset es \<Longrightarrow> 
-  ys \<noteq> xs \<Longrightarrow> dsset ys \<inter> ILC.FFVars e = {} \<Longrightarrow> 
+  ys \<noteq> xs \<Longrightarrow> dsset ys \<inter> ILC.iFV e = {} \<Longrightarrow> 
   dsset ys \<inter> ILC.IImsupp (imkSubst xs es) = {}"
 using uniformS_touchedSuper_IImsupp_imkSubst' unfolding touchedSuper_def by blast
 
@@ -267,7 +267,7 @@ assumes r: "reneqv e e'" and xs: "super xs" and rr: "reneqvS es es'"
 shows "reneqv (itvsubst (imkSubst xs es) e) (itvsubst (imkSubst xs es') e')"
 apply(rule reneqv_itvsubst[OF r])
   subgoal by (smt (verit, del_insts) Un_iff imkSubst_def inf.absorb_iff2 inf_bot_right 
-     insert_subset reneqv.simps reneqvS_def rr singleton_insert_inj_eq snth_sset touchedSuper_iVar xs)
+     insert_subset reneqv.simps reneqvS_def rr singleton_insert_inj_eq snth_sset touchedSuper_iVr xs)
   subgoal by simp
   subgoal by simp
   subgoal using rr super_uniformS_finite_touchedSuper_imkSubst uniformS_def xs by blast
@@ -282,43 +282,43 @@ using reneqv_imkSubst rr u uniformS_def3 uniform_def3 xs by blast
 
 (* Inversion/simplification rules for "uniform": *)
 
-lemma uniform_iVar[simp]:
-"uniform (iVar x) \<longleftrightarrow> (\<exists>xs. super xs \<and> x \<in> dsset xs)"
-unfolding uniform_def3 by (meson bot.extremum iVar insert_subset reneqv_iVar_casesR)
+lemma uniform_iVr[simp]:
+"uniform (iVr x) \<longleftrightarrow> (\<exists>xs. super xs \<and> x \<in> dsset xs)"
+unfolding uniform_def3 by (meson bot.extremum iVr insert_subset reneqv_iVr_casesR)
 
-lemma uniform_iLam_iff[simp]:
+lemma uniform_iLm_iff[simp]:
 assumes xs: "super xs" 
-shows "uniform (iLam xs e) \<longleftrightarrow> uniform e"
+shows "uniform (iLm xs e) \<longleftrightarrow> uniform e"
 unfolding uniform_def3  
-by (meson iLam reneqv_iLam_casesL reneqv_trans reneqv_sym xs)
+by (meson iLm reneqv_iLm_casesL reneqv_trans reneqv_sym xs)
 
 (* It is impossible to express uniformity in terms of itself alone, 
 this is why renaming equivalence was necessary... same as with parametricity etc.*)
 lemma uniform_iApp_iff:
-"uniform (iApp e es) \<longleftrightarrow> 
+"uniform (iAp e es) \<longleftrightarrow> 
  uniform e \<and> (\<forall>e e'. {e,e'} \<subseteq> sset es \<longrightarrow> reneqv e e')"
-unfolding uniform_def3 using iApp reneqv_iApp_casesL by fastforce
+unfolding uniform_def3 using iAp reneqv_iApp_casesL by fastforce
 
 lemma uniform_iApp_case:
-"uniform (iApp e es) \<Longrightarrow>
+"uniform (iAp e es) \<Longrightarrow>
  uniform e \<and> (\<forall>e' \<in> sset es. uniform e')"
 unfolding uniform_iApp_iff unfolding uniform_def3 by auto
 
 (* Other properties: *)
 
-lemma uniform_iLam_imp: "uniform (iLam xs e) \<Longrightarrow> \<exists> xs' e'. super xs' \<and> uniform e' \<and> iLam xs e = iLam xs' e'"
+lemma uniform_iLm_imp: "uniform (iLm xs e) \<Longrightarrow> \<exists> xs' e'. super xs' \<and> uniform e' \<and> iLm xs e = iLm xs' e'"
 by (smt (verit, del_insts) iterm.distinct(5) iterm.distinct(6) reneqv.simps uniform_def2)
 
 lemma super_bsmall: "super xs \<Longrightarrow> bsmall (dsset xs)"
 by (metis bsmall_def finite.emptyI finite_insert super_dsset_singl touchedSuper_def)
 
-lemma uniform_iLam_imp_avoid: 
-assumes u: "uniform (iLam xs e)" and A: "small A" "bsmall A"
-shows "\<exists> xs' e'. super xs' \<and> uniform e' \<and> iLam xs e = iLam xs' e' \<and> dsset xs' \<inter> A = {}"
+lemma uniform_iLm_imp_avoid: 
+assumes u: "uniform (iLm xs e)" and A: "small A" "bsmall A"
+shows "\<exists> xs' e'. super xs' \<and> uniform e' \<and> iLm xs e = iLm xs' e' \<and> dsset xs' \<inter> A = {}"
 proof-
-  obtain xs' e' where xs': "super xs'" and e': "uniform e'" and il: "iLam xs e = iLam xs' e'"
-  using uniform_iLam_imp[OF u] by auto
-  define B where B: "B = A \<union> dsset xs' \<union> FFVars (iLam xs e)"
+  obtain xs' e' where xs': "super xs'" and e': "uniform e'" and il: "iLm xs e = iLm xs' e'"
+  using uniform_iLm_imp[OF u] by auto
+  define B where B: "B = A \<union> dsset xs' \<union> iFV (iLm xs e)"
   have bsB: "bsmall B" unfolding B apply(intro ILC_Renaming_Equivalence.bsmall_Un)
     subgoal by fact
     subgoal using super_bsmall[OF xs'] .
@@ -351,43 +351,43 @@ proof-
     subgoal using B xxs''(2) by blast . 
 qed
      
-lemma iLam_switch_to_super: 
-assumes u: "uniform (iApp (iLam xs e1) es2)"
+lemma iLm_switch_to_super: 
+assumes u: "uniform (iAp (iLm xs e1) es2)"
 shows 
-"\<exists>xs' e1'. super xs' \<and> iLam xs e1 = iLam xs' e1' \<and> 
+"\<exists>xs' e1'. super xs' \<and> iLm xs e1 = iLm xs' e1' \<and> 
            itvsubst (imkSubst xs es2) e1 = itvsubst (imkSubst xs' es2) e1' \<and> 
-           (\<forall>e\<in>sset es2. dsset xs' \<inter> FFVars e = {})"
+           (\<forall>e\<in>sset es2. dsset xs' \<inter> iFV e = {})"
 proof- 
   obtain e2 where e2: "e2 \<in> sset es2" 
     using snth_sset by blast
   
   have uu: "\<And>e. e \<in> sset es2 \<Longrightarrow> uniform e"
   using u uniform_iApp_case by blast
-  have u': "uniform (iLam xs e1)" using u uniform_iApp_iff by blast
+  have u': "uniform (iLm xs e1)" using u uniform_iApp_iff by blast
 
-  have fves2: "touchedSuper (\<Union> (FFVars ` (sset es2))) = touchedSuper (FFVars e2) "  
-    by (metis e2 iterm.inject reneqvS_def reneqv_iApp_casesL u uniformS_def3 uniformS_touchedSuper uniform_def3)
+  have fves2: "touchedSuper (\<Union> (iFV ` (sset es2))) = touchedSuper (iFV e2) "  
+    by (metis e2 iterm.inject(2) reneqvS_def reneqv_iApp_casesL u uniformS_def3 uniformS_touchedSuper uniform_def3)
 
-  have ss: "small (\<Union> (FFVars ` (sset es2)))" 
+  have ss: "small (\<Union> (iFV ` (sset es2)))" 
   unfolding small_def apply(rule iterm.UN_bound)
     subgoal by (simp add: countable_card_ivar countable_sset)
     subgoal using iterm.set_bd_UNIV by blast .
 
-  have bs: "bsmall (\<Union> (FFVars ` (sset es2)))"
+  have bs: "bsmall (\<Union> (iFV ` (sset es2)))"
   unfolding bsmall_def fves2 unfolding bsmall_def[symmetric]  
   using bsmall_def e2 touchedSuperT_def uniform_finite_touchedUponT uu by presburger
 
-  obtain xs' e1' where xs': "super xs'" and e1': "uniform e1'" and il: "iLam xs e1 = iLam xs' e1'" 
-   "dsset xs' \<inter> (\<Union> (FFVars ` (sset es2))) = {}"
-  using bs ss u' uniform_iLam_imp_avoid by blast
+  obtain xs' e1' where xs': "super xs'" and e1': "uniform e1'" and il: "iLm xs e1 = iLm xs' e1'" 
+   "dsset xs' \<inter> (\<Union> (iFV ` (sset es2))) = {}"
+  using bs ss u' uniform_iLm_imp_avoid by blast
 
-  obtain f where f: "bij f" "|supp f| <o |UNIV::ivar set|" "id_on (ILC.FFVars (iLam xs e1)) f" 
+  obtain f where f: "bij f" "|supp f| <o |UNIV::ivar set|" "id_on (ILC.iFV (iLm xs e1)) f" 
   "dsmap f xs = xs'" "irrename f e1 = e1'" using il[unfolded iterm.inject] by auto
   
   show ?thesis apply(intro exI[of _ xs'] exI[of _ "irrename f e1"], safe)
     subgoal by fact
     subgoal unfolding il f ..
-    subgoal apply(subst irrename_eq_itvsubst_iVar')
+    subgoal apply(subst irrename_eq_itvsubst_iVr')
       subgoal by fact
       subgoal by fact
       subgoal apply(subst itvsubst_comp)
@@ -403,44 +403,44 @@ proof-
 qed
           
 lemma reneqv_head_reduction: 
-assumes r: "reneqv (iApp (iLam xs e1) es2) (iApp (iLam ys d1) ds2)"
+assumes r: "reneqv (iAp (iLm xs e1) es2) (iAp (iLm ys d1) ds2)"
 shows "reneqv (itvsubst (imkSubst xs es2) e1) (itvsubst (imkSubst ys ds2) d1)"
 proof-  (* we needed some delicate renaming lemmas, to turn 
    the bound sequences into supervariables, to allow for the nice inversion rules 
   for renaming equivalence to pop up... *)
-  have uu: "uniform (iApp (iLam xs e1) es2)" "uniform (iApp (iLam ys d1) ds2)"
+  have uu: "uniform (iAp (iLm xs e1) es2)" "uniform (iAp (iLm ys d1) ds2)"
   using r using uniform_def uniform_def2 by auto
-  obtain xs' e1' where x0: "super xs'" and x1: "iLam xs e1 = iLam xs' e1'"
+  obtain xs' e1' where x0: "super xs'" and x1: "iLm xs e1 = iLm xs' e1'"
          and x2: "itvsubst (imkSubst xs es2) e1 = itvsubst (imkSubst xs' es2) e1'"
-         and x3: "\<forall>e\<in>sset es2. dsset xs' \<inter> FFVars e = {}"
-  using uu iLam_switch_to_super by fastforce
-  hence ux': "uniform (iApp (iLam xs' e1') es2)"  
+         and x3: "\<forall>e\<in>sset es2. dsset xs' \<inter> iFV e = {}"
+  using uu iLm_switch_to_super by fastforce
+  hence ux': "uniform (iAp (iLm xs' e1') es2)"  
   using uu by auto
-  obtain ys' d1' where y0: "super ys'" and y1: "iLam ys d1 = iLam ys' d1'"
+  obtain ys' d1' where y0: "super ys'" and y1: "iLm ys d1 = iLm ys' d1'"
          and y2: "itvsubst (imkSubst ys ds2) d1 = itvsubst (imkSubst ys' ds2) d1'"
-         and y3: "\<forall>e\<in>sset ds2. dsset ys' \<inter> FFVars e = {}"
-  using uu iLam_switch_to_super by fastforce
-  hence uy': "uniform (iApp (iLam ys' d1') ds2)"  
+         and y3: "\<forall>e\<in>sset ds2. dsset ys' \<inter> iFV e = {}"
+  using uu iLm_switch_to_super by fastforce
+  hence uy': "uniform (iAp (iLm ys' d1') ds2)"  
   using uu by auto
-  have r: "reneqv (iApp (iLam xs' e1') es2) (iApp (iLam ys' d1') ds2)"
+  have r: "reneqv (iAp (iLm xs' e1') es2) (iAp (iLm ys' d1') ds2)"
   using r x1 y1 by auto 
-  hence "reneqv (iLam xs' e1') (iLam ys' d1')" and rr: "\<forall>e e'. {e,e'} \<subseteq> sset es2 \<union> sset ds2 \<longrightarrow> reneqv e e'"
+  hence "reneqv (iLm xs' e1') (iLm ys' d1')" and rr: "\<forall>e e'. {e,e'} \<subseteq> sset es2 \<union> sset ds2 \<longrightarrow> reneqv e e'"
   using reneqv_iApp_casesR by fastforce+
-  then obtain ee1' where il: "iLam ys' d1' = iLam xs' ee1'" and r: "reneqv e1' ee1'"
-  using reneqv_iLam_casesL x0 by blast
-  hence yy1: "iLam ys d1 = iLam xs' ee1'" using y1 by simp
+  then obtain ee1' where il: "iLm ys' d1' = iLm xs' ee1'" and r: "reneqv e1' ee1'"
+  using reneqv_iLm_casesL x0 by blast
+  hence yy1: "iLm ys d1 = iLm xs' ee1'" using y1 by simp
 
   have itv: "itvsubst (imkSubst xs es2) e1 = itvsubst (imkSubst xs' es2) e1'"
-  using iLam_eq_imkSubst[OF x1] .
+  using iLm_eq_imkSubst[OF x1] .
   have iitv: "itvsubst (imkSubst ys ds2) d1 = itvsubst (imkSubst xs' ds2) ee1'"
-  using iLam_eq_imkSubst[OF yy1] . 
+  using iLm_eq_imkSubst[OF yy1] . 
   
   show ?thesis unfolding itv iitv apply(rule reneqv_imkSubst)
   using r x0 rr unfolding reneqvS_def by auto
 qed
 
 lemma uniform_head_reduction: 
-assumes u: "uniform (iApp (iLam xs e1) es2)"
+assumes u: "uniform (iAp (iLm xs e1) es2)"
 shows "uniform (itvsubst (imkSubst xs es2) e1)"
 using assms unfolding uniform_def3 by (elim reneqv_head_reduction) 
 
@@ -449,7 +449,7 @@ using assms unfolding uniform_def3 by (elim reneqv_head_reduction)
 lemma uniformS_finite_touchedSuperT: 
 "uniformS es \<Longrightarrow> finite (\<Union> (touchedSuperT ` (sset es)))"
 by (metis Un_absorb equals0I 
-finite.emptyI finite_UN infinite_Un touchedSuper_iApp 
+finite.emptyI finite_UN infinite_Un touchedSuper_iAp 
 uniformS_def4 uniformS_sset_uniform uniform_finite_touchedUponT uniform_iApp_iff)
 
 (* not true (and not claimed by Mazza *)
